extraction: Create a set of microbenchmarks

src/CertifiedExtraction/ADTExamples.v
@@ -8,296 +8,6 @@ Require Import
         CertifiedExtraction.Extraction.AllInternal
         CertifiedExtraction.Extraction.Extraction.
 
-Definition MyEnvLists `{FacadeWrapper av (list W)} : Env av :=
-  (GLabelMap.empty (FuncSpec _))
-    ### ("std", "rand") ->> (Axiomatic FRandom)
-    ### ("list", "nil") ->> (Axiomatic (FacadeImplementationOfConstructor (list W) nil))
-    ### ("list", "push") ->> (Axiomatic (FacadeImplementationOfMutation_SCA (list W) cons))
-    ### ("list", "pop") ->> (Axiomatic (List_pop W))
-    ### ("list", "delete") ->> (Axiomatic (FacadeImplementationOfDestructor (list W)))
-    ### ("list", "empty?") ->> (Axiomatic (List_empty W)).
-
-Example other_test_with_adt'' `{FacadeWrapper av (list W)}:
-    sigT (fun prog => forall seq: list W, {{ [[`"arg1" <-- seq as _ ]] :: Nil }}
-                                    prog
-                                  {{ [[`"ret" <-- (List.fold_left (@Word.wminus 32) seq 0) as _]] :: Nil }} ∪ {{ StringMap.empty _ }} // MyEnvLists).
-Proof.
-  econstructor; intros.
-  repeat (compile_step || compile_loop).
-  let fop := translate_op Word.wminus in
-  apply (CompileBinopOrTest_right_inPlace fop); compile_do_side_conditions.
-Defined.
-
-Print Assumptions other_test_with_adt''. (* FIXME *)
-
-Opaque Word.wordToNat.
-Opaque Word.natToWord.
-Opaque nat_as_constant nat_as_word string_as_var.
-
-Eval compute in (extract_facade other_test_with_adt'').
-
-Require Import
-        CertifiedExtraction.Extraction.AllInternal
-        CertifiedExtraction.Extraction.External.Core
-        CertifiedExtraction.Extraction.External.Loops
-        CertifiedExtraction.Extraction.External.GenericADTMethods
-        CertifiedExtraction.Extraction.External.FacadeADTs.
-
-(* Opaque WrapInstance.            (* FIXME simpl never? *) *)
-
-Require Import FacadeLoops.
-
-Ltac defunctionalize_evar :=
-  match goal with
-  | [  |- context[?e] ] =>
-    is_evar e;
-      match type of e with
-      | ?a -> ?b => let ee := fresh in
-                  evar (ee: b);
-                    unify e (fun _:a => ee);
-                    unfold ee in *;
-                    clear ee
-      end
-  end.
-
-Ltac move_to_front var :=
-  repeat
-    lazymatch goal with         (* `at 1' prevents setoid_rewrite from modifying evars *)
-    | [  |- context[Cons ?k _ (fun _ => Cons var _ _)] ] =>
-      setoid_rewrite (TelEq_swap k var) at 1
-    | [  |- context[Cons ?k _ (fun _ => Cons (@NTSome _ _ var _) _ _)] ] =>
-      setoid_rewrite (TelEq_swap k (@NTSome _ _ var _)) at 1
-    end.
-
-Lemma CompileLoop :
-  forall `{FacadeWrapper (Value av) A} `{FacadeWrapper (Value av) A'} `{FacadeWrapper av (list A)}
-    lst init vhead vtest vlst vret fpop fempty fdealloc facadeInit facadeBody env (ext: StringMap.t (Value av)) tenv (f: Comp A' -> A -> Comp A'),
-    GLabelMap.MapsTo fpop (Axiomatic (List_pop A)) env ->
-    GLabelMap.MapsTo fempty (Axiomatic (List_empty A)) env ->
-    GLabelMap.MapsTo fdealloc (Axiomatic (FacadeImplementationOfDestructor (list A))) env ->
-    PreconditionSet tenv ext [[[vhead; vtest; vlst; vret]]] ->
-    {{ [[`vlst <-- lst as _]] :: tenv }}
-      facadeInit
-    {{ [[`vret <~~ init as _]] :: [[`vlst <-- lst as _]] :: tenv }} ∪ {{ ext }} // env ->
-    (forall head (acc: Comp A') (s: list A),
-        {{ [[`vhead <-- head as _]] :: [[`vret <~~ acc as _]] :: tenv }}
-          facadeBody
-        {{ [[`vret <~~ (f acc head) as _]] :: tenv }} ∪
-        {{ [vtest <-- wrap (bool2w false)] :: [vlst <-- wrap s] :: ext }} // env) ->
-    {{ [[`vlst <-- lst as _]] :: tenv }}
-      (Seq facadeInit (Seq (Fold vhead vtest vlst fpop fempty facadeBody) (Call (DummyArgument vtest) fdealloc (vlst :: nil))))
-    {{ [[`vret <~~ (fold_left f lst init) as _]] :: tenv }} ∪ {{ ext }} // env.
-Proof.
-  unfold DummyArgument; loop_t.
-
-  rewrite TelEq_swap by loop_t;
-    eapply CompileCallEmpty_spec; loop_t.
-
-  2:eapply CompileCallFacadeImplementationOfDestructor; loop_t.
-
-  loop_unify_with_nil_t.
-
-  loop_t.
-  clear dependent facadeInit;
-  generalize dependent init;
-  induction lst; loop_t.
-
-  move_to_front vtest;
-  apply CompileWhileFalse_Loop; loop_t.
-
-  eapply CompileWhileTrue; [ loop_t.. | ].
-
-  apply generalized @CompileCallPop; loop_t.
-
-  move_to_front vlst; apply ProgOk_Chomp_Some; loop_t.
-  move_to_front vtest; apply ProgOk_Chomp_Some; loop_t.
-  computes_to_inv; subst; defunctionalize_evar; eauto.
-
-  apply CompileCallEmpty_spec; loop_t.
-
-  loop_t.
-Qed.
-
-Lemma CompileLoop_strong :
-  forall `{FacadeWrapper (Value av) A} `{FacadeWrapper (Value av) A'} `{FacadeWrapper av (list A)}
-    lst init vhead vtest vlst vret fpop fempty fdealloc facadeInit facadeBody facadeConclude
-    env (ext: StringMap.t (Value av)) tenv tenv' (f: Comp A' -> A -> Comp A'),
-    GLabelMap.MapsTo fpop (Axiomatic (List_pop A)) env ->
-    GLabelMap.MapsTo fempty (Axiomatic (List_empty A)) env ->
-    GLabelMap.MapsTo fdealloc (Axiomatic (FacadeImplementationOfDestructor (list A))) env ->
-    PreconditionSet tenv ext [[[vhead; vtest; vlst; vret]]] ->
-    {{ [[`vlst <-- lst as _]] :: tenv }}
-      facadeInit
-    {{ [[`vret <~~ init as _]] :: [[`vlst <-- lst as _]] :: tenv }} ∪ {{ ext }} // env ->
-    {{ [[`vret <~~ (fold_left f lst init) as _]] :: tenv }}
-      facadeConclude
-    {{ [[`vret <~~ (fold_left f lst init) as _]] :: tenv' }} ∪ {{ ext }} // env ->
-    (forall head (acc: Comp A') (s: list A),
-        {{ [[`vhead <-- head as _]] :: [[`vret <~~ acc as _]] :: tenv }}
-          facadeBody
-        {{ [[`vret <~~ (f acc head) as _]] :: tenv }} ∪
-        {{ [vtest <-- wrap (bool2w false)] :: [vlst <-- wrap s] :: ext }} // env) ->
-    {{ [[`vlst <-- lst as _]] :: tenv }}
-      (Seq (Seq facadeInit (Seq (Fold vhead vtest vlst fpop fempty facadeBody) (Call (DummyArgument vtest) fdealloc (vlst :: nil)))) facadeConclude)
-    {{ [[`vret <~~ (fold_left f lst init) as _]] :: tenv' }} ∪ {{ ext }} // env.
-Proof.
-  intros.
-  eapply CompileSeq;
-    [ apply CompileLoop | eassumption ];
-    assumption.
-Qed.
-
-Definition revmap {A B} f := fun seq => @map A B f (rev seq).
-
-Lemma revmap_fold_helper:
-  forall (A A' : Type) (f : A -> A') (a : A) (vv : list A) (base : list A'),
-    revmap f (a :: vv) ++ base = revmap f vv ++ f a :: base.
-Proof.
-  unfold revmap; intros; simpl.
-  rewrite map_rev.
-  rewrite map_app.
-  simpl.
-  rewrite <- app_assoc.
-  simpl.
-  rewrite <- map_rev.
-  reflexivity.
-Qed.
-
-Lemma revmap_fold_strong :
-  forall {A B} (f: A -> B) (seq: list A) (base: list B),
-    fold_left (fun acc elem => f elem :: acc) seq base = (@revmap A B f seq) ++ base.
-Proof.
-  induction seq; simpl; intros.
-  - reflexivity.
-  - rewrite revmap_fold_helper; eauto.
-Qed.
-
-Lemma revmap_fold :
-  forall {A B} (f: A -> B) (seq: list A),
-    fold_left (fun acc elem => f elem :: acc) seq nil = @revmap A B f seq.
-Proof.
-  intros.
-  rewrite <- (app_nil_r (revmap f seq)).
-  apply revmap_fold_strong.
-Qed.
-
-Lemma revmap_fold_comp_strong :
-  forall {A B} (f: A -> B) (seq: list A) base,
-    Monad.equiv
-      (fold_left (fun cacc elem => (acc <- cacc; ret (f elem :: acc))%comp) seq base)
-      ( b <- base;
-        ret ((@revmap A B f seq) ++ b)).
-Proof.
-  intros; etransitivity.
-  2: apply Monad.computes_under_bind; intros; rewrite <- revmap_fold_strong; apply SetoidMorphisms.equiv_refl.
-
-  generalize dependent base; induction seq; simpl;
-  [ | setoid_rewrite IHseq ];
-  split; intros; computes_to_inv; subst; eauto using BindComputes.
-Qed.
-
-Lemma revmap_fold_comp :
-  forall {A B} (f: A -> B) (seq: list A),
-    Monad.equiv
-      (fold_left (fun cacc elem => (acc <- cacc; ret (f elem :: acc))%comp) seq (ret nil))
-      (ret (@revmap A B f seq)).
-Proof.
-  intros.
-  rewrite <- (app_nil_r (revmap f seq)).
-  rewrite revmap_fold_comp_strong.
-  split; intros; computes_to_inv; subst; eauto using BindComputes.
-Qed.
-
-Lemma CompileMap_ADT_strong :
-  forall {av A A'} `{FacadeWrapper av (list A)} `{FacadeWrapper av (list A')} `{FacadeWrapper av A} `{FacadeWrapper av A'}
-    (lst: list A) vhead vhead' vtest vlst vret vtmp fpop fempty falloc fdealloc fcons facadeBody facadeCoda env (ext: StringMap.t (Value av)) tenv tenv' (f: A -> A'),
-    GLabelMap.MapsTo fpop (Axiomatic (List_pop A)) env ->
-    GLabelMap.MapsTo fempty (Axiomatic (List_empty A)) env ->
-    GLabelMap.MapsTo falloc (Axiomatic (FacadeImplementationOfConstructor (list A') nil)) env ->
-    GLabelMap.MapsTo fdealloc (Axiomatic (FacadeImplementationOfDestructor (list A))) env ->
-    GLabelMap.MapsTo fcons (Axiomatic (FacadeImplementationOfMutation_ADT A' (list A') cons)) env ->
-    (* GLabelMap.MapsTo fdealloc_one (Axiomatic (FacadeImplementationOfDestructor A)) env -> *)
-    PreconditionSet tenv ext [[[vhead; vhead'; vtest; vlst; vret; vtmp]]] ->
-    {{ [[`vret <-- (revmap f lst) as _]] :: tenv }}
-      facadeCoda
-    {{ [[`vret <-- (revmap f lst) as _]] :: tenv' }} ∪ {{ ext }} // env ->
-    (forall head (s: list A) (s': list A'),
-        {{ [[`vhead <-- head as _]] :: tenv }}
-          facadeBody
-        {{ [[`vhead' <-- f head as _]] :: tenv }} ∪
-        {{ [vret <-- wrap s'] :: [vtest <-- wrap (bool2w false)] :: [vlst <-- wrap s] :: ext }} // env) ->
-    {{ [[`vlst <-- lst as _]] :: tenv }}
-      (Seq
-         (Seq
-            (Call vret falloc nil)
-            (Seq
-               (Fold vhead vtest vlst fpop fempty
-                     (Seq facadeBody
-                          (Call vtmp fcons (vret :: vhead' :: nil))))
-               (Call vtest fdealloc (vlst :: nil))))
-          facadeCoda)
-    {{ [[`vret <-- (revmap f lst) as _]] :: tenv' }} ∪ {{ ext }} // env.
-Proof.
-  intros.
-  setoid_rewrite <- revmap_fold_comp.
-  apply CompileLoop_strong; eauto.
-  PreconditionSet_t; eauto.
-  eapply (CompileCallFacadeImplementationOfConstructor (A := list A')); loop_t.
-  setoid_rewrite revmap_fold_comp; eassumption.
-  intros.
-  rewrite SameValues_Fiat_Bind_TelEq.
-  move_to_front vret.
-  apply miniChomp'; intros.
-  hoare.
-  apply ProgOk_Chomp_Some; loop_t; defunctionalize_evar; eauto.
-  apply CompileCallFacadeImplementationOfMutation_ADT; compile_do_side_conditions.
-Qed.
-
-Lemma CompileMap_SCA_strong :
-  forall {av A} `{FacadeWrapper av (list A)} `{FacadeWrapper av (list W)} `{FacadeWrapper av A}
-    (lst: list A) vhead vhead' vtest vlst vret vtmp fpop fempty falloc fdealloc fcons facadeBody facadeCoda env (ext: StringMap.t (Value av)) tenv tenv' (f: A -> W),
-    GLabelMap.MapsTo fpop (Axiomatic (List_pop A)) env ->
-    GLabelMap.MapsTo fempty (Axiomatic (List_empty A)) env ->
-    GLabelMap.MapsTo falloc (Axiomatic (FacadeImplementationOfConstructor (list W) nil)) env ->
-    GLabelMap.MapsTo fdealloc (Axiomatic (FacadeImplementationOfDestructor (list A))) env ->
-    GLabelMap.MapsTo fcons (Axiomatic (FacadeImplementationOfMutation_SCA (list W) cons)) env ->
-    (* GLabelMap.MapsTo fdealloc_one (Axiomatic (FacadeImplementationOfDestructor A)) env -> *)
-    PreconditionSet tenv ext [[[vhead; vhead'; vtest; vlst; vret; vtmp]]] ->
-    {{ [[`vret <-- (revmap f lst) as _]] :: tenv }}
-      facadeCoda
-    {{ [[`vret <-- (revmap f lst) as _]] :: tenv' }} ∪ {{ ext }} // env ->
-    (forall head (s: list A) (s': list W),
-        {{ [[`vhead <-- head as _]] :: tenv }}
-          facadeBody
-        {{ [[`vhead' <-- f head as _]] :: tenv }} ∪
-        {{ [vret <-- wrap s'] :: [vtest <-- wrap (bool2w false)] :: [vlst <-- wrap s] :: ext }} // env) ->
-    {{ [[`vlst <-- lst as _]] :: tenv }}
-      (Seq
-         (Seq
-            (Call vret falloc nil)
-            (Seq
-               (Fold vhead vtest vlst fpop fempty
-                     (Seq facadeBody
-                          (Call (DummyArgument vtmp) fcons (vret :: vhead' :: nil))))
-               (Call (DummyArgument vtest) fdealloc (vlst :: nil))))
-          facadeCoda)
-    {{ [[`vret <-- (revmap f lst) as _]] :: tenv' }} ∪ {{ ext }} // env.
-Proof.
-  intros.
-  setoid_rewrite <- revmap_fold_comp.
-  apply CompileLoop_strong; eauto.
-  PreconditionSet_t; eauto.
-  eapply (CompileCallFacadeImplementationOfConstructor (A := list W)); loop_t.
-  setoid_rewrite revmap_fold_comp; eassumption.
-  intros.
-  rewrite SameValues_Fiat_Bind_TelEq.
-  move_to_front vret.
-  apply miniChomp'; intros.
-  hoare.
-  apply ProgOk_Chomp_Some; loop_t; defunctionalize_evar; eauto.
-  apply CompileCallFacadeImplementationOfMutation_SCA; unfold DummyArgument; compile_do_side_conditions.
-Qed.
-
 Parameter TSearchTerm : Type.
 Parameter TAcc : Type.
 Definition av := (list W + TSearchTerm + TAcc)%type.
@@ -313,107 +23,20 @@ Definition MyEnvListsB : Env (list W + TSearchTerm + TAcc) :=
     ### ("search", "delete!") ->> (Axiomatic (FacadeImplementationOfDestructor TSearchTerm))
     ### ("acc", "delete!") ->> (Axiomatic (FacadeImplementationOfDestructor TAcc)).
 
-Ltac compile_loop :=
-  match_ProgOk
-    ltac:(fun prog pre post ext env =>
-            let vtest := gensym "test" in
-            let vhead := gensym "head" in
-            match constr:(pre, post) with
-            | (Cons (NTSome ?vseq) (ret ?seq) ?tenv, Cons (NTSome ?vret) (List.fold_left _ ?seq _) ?tenv') =>
-              apply (CompileLoop_strong (vtest := vtest) (vhead := vhead)); try compile_do_side_conditions
-            | (Cons (NTSome ?vseq) (ret ?seq) ?tenv, Cons (NTSome ?vret) (ret (List.fold_left _ ?seq _)) ?tenv') =>
-              (* FIXME rename and generalize to different tenvs *)
-              apply (FacadeLoops.CompileLoop CompileLoop_strong (vtest := vtest) (vhead := vhead)); try compile_do_side_conditions
-            end).
 
-Ltac compile_destructor :=
-  match_ProgOk
-    ltac:(fun prog pre post ext env =>
-            let vtmp := gensym "tmp" in
-            match constr:(pre, post) with
-            | (Cons _ _ (fun _ => ?tenv), ?tenv) =>
-              apply (CompileCallFacadeImplementationOfDestructor (vtmp := DummyArgument vtmp))
-            | (Cons _ ?v (fun _ => ?tenv), ?tenv') =>
-              match tenv' with
-              | context[v] => fail 1
-              | _ => eapply CompileSeq; [ apply (CompileCallFacadeImplementationOfDestructor (vtmp := DummyArgument vtmp)) | ]
-              end
-            end; try compile_do_side_conditions).
-
-Ltac compile_miniChomp :=
-  match_ProgOk
-    ltac:(fun prog pre post ext env =>
-            match post with
-            | Cons NTNone ?v ?tenv' =>
-              match pre with
-              | context[Cons ?k v _] =>
-                move_to_front k;
-                  apply miniChomp'
-              end
-            end).
-
-Example other_test_with_adt''':
-  sigT (fun prog => forall (searchTerm: TSearchTerm) (init: TAcc),
-            {{ [[`"search" <-- searchTerm as _]] :: [[`"init" <-- init as _]] :: (@Nil av) }}
-              prog
-            {{ [[`"ret" <~~  ( seq <- {s: list W | True };
-                             fold_left (fun acc elem =>
-                                          acc <- acc;
-                                          { x: W | Word.wlt (Word.wplus acc elem) x })
-                                       seq (ret (Word.natToWord 32 0: W))) as _]] :: (@Nil av) }} ∪ {{ StringMap.empty (Value av) }} // MyEnvListsB).
-Proof.
-  econstructor; intros.
-
-  repeat setoid_rewrite SameValues_Fiat_Bind_TelEq.
-
-  (* FXIME compile_do_alloc should use Transitivity_Name' *)
-  eapply ProgOk_Transitivity_Name' with "seq".
-
-  instantiate (1 := Skip).       (* FIXME alloc *)
-  admit.
-
-  compile_miniChomp.
-  compile_step.
-  compile_loop.
-  compile_step.
-
-  repeat compile_step.
-
-  compile_destructor.
-  compile_destructor.
-
-  compile_step.
-  repeat setoid_rewrite SameValues_Fiat_Bind_TelEq.
-
-  compile_do_extend_scalar_lifetime.
-  compile_step.
-  compile_step.
-  (* FIXME compile_do_alloc shouldn't be called here. *)
-  compile_miniChomp.
-  compile_step.
-  compile_step.
-
-  instantiate (1 := Skip).
-  admit.
-Defined.
-
-Opaque DummyArgument.
-
-Eval compute in (extract_facade other_test_with_adt''').
-
-Lemma SameValues_Fiat_Bind_TelEq_Pair :
-  forall {av A1 A2 B} key compA compB tail ext,
-    TelEq ext
-          (Cons (av := av) key (@Bind (A1 * A2) B compA compB) tail)
-          (Cons NTNone compA (fun a => Cons NTNone (ret (fst a)) (fun a1 => Cons NTNone (ret (snd a)) (fun a2 => Cons key (compB (a1, a2)) tail)))).
-Proof.
-  unfold TelEq;
-  repeat match goal with
-         | _ => progress subst
-         | _ => progress SameValues_Fiat_t_step
-         | _ => rewrite <- surjective_pairing in *
-         end.
-Qed.
+(* Ltac compile_destructor := *)
+(*   match_ProgOk *)
+(*     ltac:(fun prog pre post ext env => *)
+(*             let vtmp := gensym "tmp" in *)
+(*             match constr:(pre, post) with *)
+(*             | (Cons _ _ (fun _ => ?tenv), ?tenv) => *)
+(*               apply (CompileCallFacadeImplementationOfDestructor (vtmp := DummyArgument vtmp)) *)
+(*             | (Cons _ ?v (fun _ => ?tenv), ?tenv') => *)
+(*               match tenv' with *)
+(*               | context[v] => fail 1 *)
+(*               | _ => eapply CompileSeq; [ apply (CompileCallFacadeImplementationOfDestructor (vtmp := DummyArgument vtmp)) | ] *)
+(*               end *)
+(*             end. *)
 
 Require Import Fiat.QueryStructure.Implementation.DataStructures.BagADT.QueryStructureImplementation Fiat.QueryStructure.Automation.Common Fiat.QueryStructure.Specification.Representation.Schema.
 Require Import Coq.Vectors.Fin.
@@ -421,154 +44,11 @@ Require Import Coq.Vectors.Fin.
 (* Notation "'BIND' !! A !! B !! C" := (@Bind A B C) (at level 1). *)
 (* Notation "x { A } <- y ; z" := (Bind y (fun x: A => z)) (at level 1). *)
 
-Lemma ProgOk_Transitivity_Name_Pair :
-  forall {av A1 A2} `{FacadeWrapper av A1} `{FacadeWrapper av A2} {ext env}
-    vfst vsnd tenv tenv' (pair: Comp (A1 * A2)) prog d1 d2,
-    {{ tenv }}
-      prog
-    {{ [[pair as p]] :: [[`vfst <-- fst p as p1]] :: [[`vsnd <-- snd p as p2]] :: tenv' p1 p2 }} ∪ {{ext}} // env ->
-    {{ [[pair as p]] :: [[`vfst <-- fst p as p1]] :: [[`vsnd <-- snd p as p2]] :: tenv' p1 p2 }}
-      d1
-    {{ [[pair as p]] :: [[ret (fst p) as p1]] :: [[`vsnd <-- snd p as p2]] :: tenv' p1 p2 }} ∪ {{ext}} // env ->
-    {{ [[pair as p]] :: [[ret (fst p) as p1]] :: [[`vsnd <-- snd p as p2]] :: tenv' p1 p2 }}
-      d2
-    {{ [[pair as p]] :: [[ret (fst p) as p1]] :: [[ret (snd p) as p2]] :: tenv' p1 p2 }} ∪ {{ext}} // env ->
-    {{ tenv }}
-      Seq prog (Seq d1 d2)
-    {{ [[pair as p]] :: [[ret (fst p) as p1]] :: [[ret (snd p) as p2]] :: tenv' p1 p2 }} ∪ {{ext}} // env.
-Proof.
-  repeat hoare.
-Qed.
-
-Lemma CompileDeallocADT_discretely : (* TODO create a specialized version that hardcodes the deallocation call *)
-  forall {av A} {env ext} (k: NameTag av A) comp tenv tenv' prog dealloc,
-    {{ [[k <~~ comp as kk]] :: tenv kk }}
-      prog
-      {{ [[k <~~ comp as kk]] :: tenv' kk }} ∪ {{ext}} // env ->
-    {{ [[k <~~ comp as kk]] :: tenv' kk }}
-      dealloc
-      {{ [[comp as kk]] :: tenv' kk }} ∪ {{ext}} // env ->
-    {{ [[k <~~ comp as kk]] :: tenv kk }}
-      (Seq prog dealloc)
-      {{ [[comp as kk]] :: tenv' kk }} ∪ {{ext}} // env.
-Proof.
-  repeat hoare.
-Qed.
-
-Lemma CompileDeallocADT_discretely' : (* TODO create a specialized version that hardcodes the deallocation call *)
-  forall {av A} {env ext} (k: NameTag av A) v tenv tenv' prog dealloc,
-    {{ [[k <-- v as _]] :: tenv }}
-      prog
-    {{ [[k <-- v as _]] :: tenv' }} ∪ {{ext}} // env ->
-    {{ [[k <-- v as _]] :: tenv' }}
-      dealloc
-    {{ tenv' }} ∪ {{ext}} // env ->
-    {{ [[k <-- v as _]] :: tenv }}
-      (Seq prog dealloc)
-    {{ tenv' }} ∪ {{ext}} // env.
-Proof.
-  repeat hoare.
-Qed.
-
 Definition FinToWord {N: nat} (n: Fin.t N) :=
   Word.natToWord 32 (proj1_sig (Fin.to_nat n)).
 
 Definition FitsInW {N: nat} (n: Fin.t N) :=
   Word.wordToNat (FinToWord n) = proj1_sig (Fin.to_nat n).
-
-Ltac compile_chomp :=
-  match_ProgOk
-    ltac:(fun prog pre post ext env =>
-            match pre with    (* FIXME could be generalized beyond the first binding *)
-            | Cons ?k ?v ?tenv =>
-              match post with
-              | Cons k v _ => fail 1
-              | context[Cons k v _] => move_to_front k
-              end
-            end).
-
-Ltac compile_dealloc_useless :=  (* FIXME used? *)
-  match_ProgOk
-    ltac:(fun prog pre post ext env =>
-            match pre with
-            | Cons ?k ?v ?tenv =>
-              match post with
-              | context[k] => fail 1 "k appears in conclusion"
-              | context[v] => fail 1 "v appears in conclusion"
-              | _ => apply CompileDeallocSCA_discretely
-              | _ => apply CompileDeallocADT_discretely
-              | _ => apply CompileDeallocADT_discretely'
-              end
-            end).
-
-Ltac _compile_CallGetAttribute :=
-  match_ProgOk
-    ltac:(fun prog pre post ext env =>
-            match constr:(pre, post) with
-            | (Cons (NTSome ?vsrc) (ret ?src) ?tenv,
-               Cons (NTSome ?vtarget) (ret (GetAttributeRaw ?src ?index)) ?tenv') =>
-              let vindex := gensym "index" in
-              eapply CompileSeq with ([[`vindex <-- FinToWord index as _]]
-                                        :: [[`vsrc <-- src as src]]
-                                        :: (tenv src));
-                [ | match_ProgOk
-                      ltac:(fun prog' _ _ _ _ =>
-                              unify prog' (Call vtarget ("ext", "GetAttribute")
-                                                (vsrc :: vindex :: nil))) ]
-            end).
-
-Ltac _compile_map :=
-  match_ProgOk
-    ltac:(fun prog pre post ext env =>
-            let vhead := gensym "head" in
-            let vhead' := gensym "head'" in
-            let vtest := gensym "test" in
-            let vtmp := gensym "tmp" in
-            match constr:(pre, post) with
-            | (Cons (NTSome ?vseq) (ret ?seq) ?tenv, Cons (NTSome ?vret) (ret (revmap _ ?seq')) ?tenv') =>
-              unify seq seq';
-                first [
-                    apply (CompileMap_SCA_strong seq (vhead := vhead) (vhead' := vhead') (vtest := vtest) (vtmp := DummyArgument vtmp)) |
-                    apply (CompileMap_ADT_strong seq (vhead := vhead) (vhead' := vhead') (vtest := vtest) (vtmp := DummyArgument vtmp)) ];
-                try compile_do_side_conditions
-            end).
-
-
-  Ltac facade_if_helper ::=     (* Add an eauto 3 to prevent spurious existentials from popping up *)
-  match goal with
-  | H:is_true ?st (isTrueExpr ?k),
-    H':StringMap.MapsTo ?k (wrap (bool2w ?test)) ?st
-    |- _ => learn (is_true_isTrueExpr H H')
-  | H:is_false ?st (isTrueExpr ?k),
-    H':StringMap.MapsTo ?k (wrap (bool2w ?test)) ?st
-    |- _ => learn (is_false_isTrueExpr H H')
-  | _ => solve
-  [ eauto 3 using isTrueExpr_is_false, isTrueExpr_is_true  with SameValues_db ]
-  | _ => solve
-  [ eauto using isTrueExpr_is_false, isTrueExpr_is_true  with SameValues_db ]
-  end.
-
-Lemma CompileIf :
-  forall {av A} k tmp (gallinaTest: bool) (gallinaT gallinaF: Comp A) facadeTest facadeT facadeF
-    env (ext: StringMap.t (Value av)) tenv tenv',
-    tmp ∉ ext ->
-    NotInTelescope tmp tenv ->
-    {{ tenv }}
-      facadeTest
-    {{ [[`tmp <-- (bool2w gallinaTest) as _]]::tenv }} ∪ {{ ext }} // env ->
-    {{ [[`tmp <-- (bool2w gallinaTest) as _]]::tenv }}
-      facadeT
-    {{ [[`tmp <-- (bool2w gallinaTest) as _]]::[[k <~~ gallinaT as v]]::tenv' v }} ∪ {{ ext }} // env ->
-    {{ [[`tmp <-- (bool2w gallinaTest) as _]]::tenv }}
-      facadeF
-    {{ [[`tmp <-- (bool2w gallinaTest) as _]]::[[k <~~ gallinaF as v]]::tenv' v }} ∪ {{ ext }} // env ->
-    {{ tenv }}
-      (Seq facadeTest (DFacade.If (isTrueExpr tmp) facadeT facadeF))
-    {{ [[k <~~ if gallinaTest then gallinaT else gallinaF as v]]::tenv' v }} ∪ {{ ext }} // env.
-Proof.
-  intros; hoare.
-  repeat (SameValues_Facade_t_step || facade_if_helper).
-Qed.
 
 Set Printing All.
 Set Printing Depth 1000.
@@ -1174,45 +654,6 @@ Definition MethodOfInterest :=
                                          (Vector.cons Type ProcessScheduler.State (S O) (Vector.cons Type W O (Vector.nil Type)))))))
                              a)))))).
 
-Lemma SameValues_remove_SCA:
-  forall (av0 : Type) (tenv' : Telescope av0)
-    (ext : StringMap.t (Value av0)) (k : StringMap.key)
-    (final_state : State av0) (x : W),
-    StringMap.MapsTo k (wrap x) final_state ->
-    StringMap.remove (elt:=Value av0) k final_state ≲ tenv' ∪ ext ->
-    final_state ≲ tenv' ∪ ext.
-Proof.
-  induction tenv'; simpl; intros.
-  - rewrite (add_redundant_cancel H).
-    rewrite <- add_remove_cancel; try reflexivity.
-    apply WeakEq_pop_SCA.
-    apply StringMap.remove_1; reflexivity.
-    assumption.
-  - destruct key; repeat cleanup.
-    + eauto.
-    + SameValues_Fiat_t.
-      StringMap_t.
-      rewrite remove_mapsto_iff in *.
-      cleanup.
-      StringMap_t.
-      repeat cleanup.
-      eapply H.
-      2: rewrite remove_remove_comm; eauto.
-      rewrite remove_mapsto_iff in *; eauto.
-Qed.
-
-Hint Resolve SameValues_remove_SCA : SameValues_db.
-
-Lemma CompileDeallocSCA_discretely :
-  forall {av} (tenv tenv': Telescope av) ext env k (v: Comp W) prog,
-    k ∉ ext ->
-    NotInTelescope k tenv ->
-    {{ [[`k <~~ v as _]] :: tenv }} prog {{ [[`k <~~ v as _]] :: tenv' }} ∪ {{ ext }} // env ->
-    {{ [[`k <~~ v as _]] :: tenv }} prog {{ tenv' }} ∪ {{ ext }} // env.
-Proof.
-  SameValues_Facade_t.
-Qed.
-
 Print Type1.
 
 Definition av' := (list W + Type1 +
@@ -1238,6 +679,23 @@ Definition MyEnvListsC : Env av' :=
     ### ("RawTuple", "delete!") ->> (Axiomatic (FacadeImplementationOfDestructor (@RawTuple heading))).
 
 Check MethodOfInterest.
+
+Ltac _compile_CallGetAttribute :=
+  match_ProgOk
+    ltac:(fun prog pre post ext env =>
+            match constr:(pre, post) with
+            | (Cons (NTSome ?vsrc) (ret ?src) ?tenv,
+               Cons (NTSome ?vtarget) (ret (GetAttributeRaw ?src ?index)) ?tenv') =>
+              let vindex := gensym "index" in
+              eapply CompileSeq with ([[`vindex <-- FinToWord index as _]]
+                                        :: [[`vsrc <-- src as src]]
+                                        :: (tenv src));
+                [ | match_ProgOk
+                      ltac:(fun prog' _ _ _ _ =>
+                              unify prog' (Call vtarget ("ext", "GetAttribute")
+                                                (vsrc :: vindex :: nil))) ]
+            end).
+
 
 Ltac _compile_CallBagFind :=
   match_ProgOk
@@ -1282,179 +740,22 @@ Ltac _compile_CallBagInsert :=
                  end
              end).
 
-Ltac _compile_chomp :=         (* This is a weak version of the real compile_chomp, which is too slow *)
-  match_ProgOk
-    ltac:(fun prog pre post ext env =>
-            match constr:(pre, post) with
-            | (Cons ?k ?v ?tenv, Cons ?k' ?v' ?tenv') =>
-              unify k k'; unify v v';
-              match k with
-              | NTNone => apply ProgOk_Chomp_None
-              | _ => apply ProgOk_Chomp_Some
-              end
-            end).
-
-Ltac tenv_mentions env v :=
-  first [ match env with
-          | context[?vv] => first [ is_evar vv; fail 1
-                                 | unify v vv; fail 2 ]
-          | _ => idtac
-          end; fail 1 | idtac ].
-
-Ltac tenv_mentions_fast env v :=
-  lazymatch v with
-  | ?f => match env with context[f] => idtac end
-  | ?f ?a => match env with context[f ?a'] => unify a a' end
-  | ?f ?a ?b => match env with context[f ?a' ?b'] => unify a a'; unify b b' end
-  | ?f ?a ?b ?c => match env with context[f ?a' ?b' ?c'] => unify a a'; unify b b'; unify c c' end
-  | ?f ?a ?b ?c ?d => match env with context[f ?a' ?b' ?c' ?d'] => unify a a'; unify b b'; unify c c'; unify d d' end
-  end.
-
-Ltac _compile_destructor_unsafe vtmp tenv tenv' :=
-  (apply CompileDeallocSCA_discretely ||
-   first [ unify tenv tenv';
-           apply (CompileCallFacadeImplementationOfDestructor (vtmp := DummyArgument vtmp))
-         | eapply CompileSeq;
-           [ apply (CompileCallFacadeImplementationOfDestructor (vtmp := DummyArgument vtmp)) | ] ]);
-  try compile_do_side_conditions.
-
-Ltac _compile_destructor :=
-  match_ProgOk
-     ltac:(fun prog pre post ext env =>
-             let vtmp := gensym "tmp" in
-             match pre with
-             | Cons _ ?v (fun _ => ?tenv) =>
-               match tenv with
-               | context[post] => _compile_destructor_unsafe vtmp tenv post
-               | _ => unify tenv post; _compile_destructor_unsafe vtmp tenv post
-               | _ => lazymatch v with
-                 | ret ?vv => first [ tenv_mentions_fast post vv; fail 1
-                                   | _compile_destructor_unsafe vtmp tenv post ]
-                 | ?vv => first [ tenv_mentions_fast post vv; fail 1
-                               | _compile_destructor_unsafe vtmp tenv post ]
-                 end
-               end
-             end).
-
-Ltac _compile_skip :=
-  match_ProgOk
-    ltac:(fun prog pre post ext env =>
-            match constr:(pre, post) with
-            | (?tenv, ?tenv') => not_evar tenv; not_evar tenv'; unify tenv tenv'; apply CompileSkip
-            end).
-
-Ltac _compile_if :=
-  match_ProgOk
-    ltac:(fun prog pre post ext env =>
-            match constr:(pre, post) with
-            | (_, Cons _ (if _ then _ else _) _) =>
-              let vtmp := gensym "test" in
-              apply (CompileIf (tmp := "test"))
-            end).
-
-Ltac __compile_prepare_chomp tenv tenv' :=
-  match tenv with
-  | Cons ?k ?v _ =>
-    match tenv' with
-    | Cons ?k' ?v' _ =>
-      unify k k'; unify v v';
-      fail 1 (* Nothing to do: can already chomp *)
-    | Cons _ _ (fun _ => ?tail) =>
-      unify tenv tail; idtac;
-      fail 1 (* This is a job for deallocation, not chomping *)
-    | context[Cons k v _] =>
-      move_to_front k
-    end
-  end.
-
-Ltac _compile_prepare_chomp :=
-  match_ProgOk
-    ltac:(fun prog pre post ext env =>
-            is_evar prog;
-            first [ __compile_prepare_chomp pre post
-                  | __compile_prepare_chomp post pre ]).
-
 Arguments wrap : simpl never.
-
-Ltac useless_binder term :=
-  lazymatch term with
-  | (fun _ => ?body) => let capture := body in idtac
-  end.
-
-Ltac _compile_rewrite :=
-  (* setoid_rewrite at the speed of light *)
-  match_ProgOk
-    ltac:(fun prog pre post ext env =>
-            match constr:(pre, post) with
-            | context[Cons ?k (ret _) ?tail] =>
-              first [ useless_binder tail; fail 1 |
-                      match k with
-                      | NTSome _ => setoid_rewrite Propagate_ret
-                      | NTNone => setoid_rewrite Propagate_anonymous_ret
-                      end ]
-            | context[Cons _ (Bind _ _) _] => setoid_rewrite SameValues_Fiat_Bind_TelEq
-            end).
-
-Ltac _compile_step :=
-  match goal with
-  | _ => progress subst; idtac "progress subst"
-  | _ => progress intros; idtac "progress intros"
-  | _ => progress computes_to_inv; idtac "progress computes_to_inv"
-  | _ => _compile_rewrite; idtac "_compile_rewrite"
-  | _ => compile_do_side_conditions; idtac "compile_do_side_conditions"
-  | _ => _compile_skip; idtac "_compile_skip"
-  | _ => _compile_map; idtac "_compile_map"
-  | _ => _compile_CallBagFind; idtac "_compile_CallBagFind"
-  | _ => _compile_CallBagInsert; idtac "_compile_CallBagInsert"
-  | _ => _compile_CallGetAttribute; idtac "_compile_CallGetAttribute"
-  | _ => _compile_destructor; idtac "_compile_destructor"
-  | _ => _compile_chomp; idtac "_compile_chomp"
-  | _ => _compile_prepare_chomp; idtac "_compile_prepare_chomp"
-  | _ => _compile_if; idtac "_compile_if"
-  | _ => compile_simple; idtac "compile_simple"
-  | _ => progress simpl; idtac "progress simpl"
-  end.
-
-Ltac _compile :=
-  repeat _compile_step.
-
-Ltac _compile_random :=
-  match_ProgOk
-    ltac:(fun prog pre post ext env =>
-            match constr:(pre, post) with
-            | (?tenv, Cons NTNone Random ?tenv') =>
-              let vrandom := gensym "random" in
-              apply ProgOk_Transitivity_Name with vrandom;
-                [ call_tactic_after_moving_head_binding_to_separate_goal
-                    ltac:(apply CompileCallRandom) | apply miniChomp' ] (* FIXME do deallocation here *)
-            end).
-
-Ltac compile_do_side_conditions_internal ::=
-  repeat cleanup; PreconditionSet_t;
-   match goal with
-   | _ => exact I
-   | |- _ <> _ => discriminate 1
-   | |- _ ∉ _ => decide_not_in
-   | |- NotInTelescope _ _ => decide_NotInTelescope
-   | |- StringMap.find _ _ = Some _ => decide_mapsto_maybe_instantiate
-   | |- StringMap.MapsTo _ _ _ => decide_mapsto_maybe_instantiate
-   | |- GLabelMap.MapsTo _ _ _ =>
-         GLabelMapUtils.decide_mapsto_maybe_instantiate
-   end.
 
 Example random_test_with_adt :
   Facade program implementing ( x <- Random;
                                 ret (if IL.weqb x 0 then
-                                       (Word.natToWord 32 1 : W) :: nil
+                                       (Word.natToWord 32 1) :: nil
                                      else
                                        x :: nil)) with MyEnvW.
 Proof.
   Time compile_step.
-  repeat (_compile_random || compile_mutation_alloc || compile_constructor || _compile_step || match_ProgOk compile_rewrite).
-  (* FIXME try the side conditions before subst and computes_to_inv? *)
+  repeat (_compile_step || _compile_random).
 Defined.
 
 Eval compute in (extract_facade random_test_with_adt).
+
+(* Require Import Utf8 FIXME remove *)
 
 Definition Remembered {A} (a : A) := a.
 
@@ -1498,6 +799,59 @@ Ltac unset_values :=
 (*                end *)
 (*              end). *)
 
+
+
+Example other_test_with_adt''':
+  sigT (fun prog => forall (searchTerm: TSearchTerm) (init: TAcc),
+            {{ [[`"search" <-- searchTerm as _]] :: [[`"init" <-- init as _]] :: (@Nil av) }}
+              prog
+            {{ [[`"ret" <~~  ( seq <- {s: list W | True };
+                             fold_left (fun acc elem =>
+                                          acc <- acc;
+                                          { x: W | Word.wlt (Word.wplus acc elem) x })
+                                       seq (ret (Word.natToWord 32 0: W))) as _]] :: (@Nil av) }} ∪ {{ StringMap.empty (Value av) }} // MyEnvListsB).
+Proof.
+  econstructor; intros.
+
+  (* repeat setoid_rewrite SameValues_Fiat_Bind_TelEq. *)
+
+  _compile.
+
+  eapply ProgOk_Transitivity_Name' with "seq".
+  instantiate (1 := Skip).       (* FIXME alloc *)
+  admit.
+  compile_miniChomp.
+
+  _compile.
+  compile_loop.
+
+  _compile.
+  _compile.
+  _compile.
+
+  compile_do_extend_scalar_lifetime.
+  _compile.
+
+  compile_miniChomp.
+  _compile.
+
+  instantiate (1 := Skip); admit.
+Defined.
+
+Eval compute in (extract_facade other_test_with_adt''').
+
+Example other_test_with_adtB'' `{FacadeWrapper av (list W)}:
+    sigT (fun prog => forall seq: list W, {{ [[`"arg1" <-- seq as _ ]] :: Nil }}
+                                    prog
+                                  {{ [[`"ret" <-- (List.fold_left (@Word.wminus 32) seq 0) as _]] :: Nil }} ∪ {{ StringMap.empty _ }} // MyEnvLists).
+Proof.
+  econstructor; intros.
+  Print Ltac compile_loop.
+  repeat (compile_step || compile_loop).
+  let fop := translate_op Word.wminus in
+  apply (CompileBinopOrTest_right_inPlace fop); compile_do_side_conditions.
+Defined.
+
 Example compile2 :
   sigT (fun prog => forall r_n d d0,
             {{ [[`"r_n" <-- r_n as _ ]] :: [[`"d" <-- d as _]] :: [[`"d0" <-- d0 as _]] :: Nil }}
@@ -1526,43 +880,45 @@ Proof.
   eexists; intros.
   unfold MethodOfInterest.
 
-  _compile_step.
-  _compile_step.
-  _compile_step.
-  
-  _compile_step.
-  _compile_step.
-  _compile_step.
-  _compile_step.
-  _compile_step.
-  _compile_step.
-  _compile_step.
-  _compile_step.
-  _compile_step.
-  _compile_step.
-  _compile_step.
-  _compile_step.
-  _compile_step.
-  _compile_step.
-  _compile_step.
-  _compile_step.
-  _compile_step.
-  _compile_step.
-  _compile_step.
-  _compile_step.
-  _compile_step.
-  _compile_step.
-  _compile_step.
-  _compile_step.
+  Ltac _compile_CallBagFind ::=
+    match_ProgOk
+      ltac:(fun prog pre post ext env =>
+              match constr:(pre, post) with
+              | (Cons (NTSome ?vdb) (ret ?db) (fun _ => Cons (NTSome ?vd) (ret ?d) ?tenv),
+                 Cons NTNone (CallBagMethod ?id BagFind ?db _) ?tenv') =>
+                let vsnd := gensym "snd" in
+                let vtmp := gensym "tmp" in
+                match post with
+                | Cons NTNone ?bf _ =>
+                  eapply CompileSeq with ([[bf as retv]]
+                                            :: [[`vdb <-- Refinements.UpdateIndexedRelation
+                                                 (QueryStructureSchema.QueryStructureSchemaRaw SchedulerSchema)
+                                                 (icons3 SearchUpdateTerm inil3) db F1 (fst retv)
+                                                 as _]]
+                                            :: [[`vsnd <-- snd retv as s]]
+                                            :: [[`vd <-- d as _]]
+                                            :: (tenv d));
+                    [ match_ProgOk
+                        ltac:(fun prog' _ _ _ _ =>
+                                unify prog' (Call (DummyArgument vtmp) ("ext", "BagFind")
+                                                  (vsnd :: vdb :: vd :: nil))) (* FIXME *) | ]
+                end
+              end).
 
-  
-  Time repeat (_compile_step || change (ilist2.ilist2_hd (ilist2.icons2 head ilist2.inil2)) with head).
+  Lemma map_rev_def :
+    forall {A B} f seq,
+      @map A B f (rev seq) = revmap f seq.
+  Proof.
+    intros; reflexivity.
+  Qed.
+
+  Time repeat (_compile_step || setoid_rewrite map_rev_def).
   admit.
   admit.
 Defined.
 
 Opaque DummyArgument.
-Eval compute in (extract_facade compile).
+Definition compiled := Eval compute in (extract_facade compile).
 
 Example other_test_with_adt''''' :
     sigT (fun prog => forall seq seq', {{ [[`"arg1" <-- seq as _ ]] :: [[`"arg2" <-- seq' as _]] :: Nil }}
