src/CertifiedExtraction/Microbenchmarks.v
@@ -1,0 +1,1235 @@
+Require Import
+        CertifiedExtraction.Core
+        CertifiedExtraction.FacadeUtils
+        CertifiedExtraction.StringMapUtils
+        CertifiedExtraction.Examples
+        CertifiedExtraction.Extraction.AllInternal
+        CertifiedExtraction.Extraction.Extraction.
+
+(* FIXME move *)
+
+
+Require Import
+        CertifiedExtraction.Extraction.AllInternal
+        CertifiedExtraction.Extraction.External.Core
+        CertifiedExtraction.Extraction.External.Loops
+        CertifiedExtraction.Extraction.External.GenericADTMethods
+        CertifiedExtraction.Extraction.External.FacadeADTs.
+
+(* Opaque WrapInstance.            (* FIXME simpl never? *) *)
+
+Require Import FacadeLoops.
+
+Ltac defunctionalize_evar :=
+  match goal with
+  | [  |- context[?e] ] =>
+    is_evar e;
+      match type of e with
+      | ?a -> ?b => let ee := fresh in
+                  evar (ee: b);
+                    unify e (fun _:a => ee);
+                    unfold ee in *;
+                    clear ee
+      end
+  end.
+
+Ltac move_to_front var :=
+  repeat
+    lazymatch goal with         (* `at 1' prevents setoid_rewrite from modifying evars *)
+    | [  |- context[Cons ?k _ (fun _ => Cons var _ _)] ] => setoid_rewrite (TelEq_swap k var) at 1
+    | [  |- context[Cons ?k _ (fun _ => Cons (@NTSome _ _ var _) _ _)] ] => setoid_rewrite (TelEq_swap k (@NTSome _ _ var _)) at 1
+    end.
+
+Lemma CompileLoopBase :
+  forall `{FacadeWrapper (Value av) A} `{FacadeWrapper (Value av) A'} `{FacadeWrapper av (list A)}
+    lst init vhead vtest vlst vret fpop fempty fdealloc facadeBody env (ext: StringMap.t (Value av)) tenv (f: Comp A' -> A -> Comp A'),
+    GLabelMap.MapsTo fpop (Axiomatic (List_pop A)) env ->
+    GLabelMap.MapsTo fempty (Axiomatic (List_empty A)) env ->
+    GLabelMap.MapsTo fdealloc (Axiomatic (FacadeImplementationOfDestructor (list A))) env ->
+    PreconditionSet tenv ext [[[vhead; vtest; vlst; vret]]] ->
+    (forall head (acc: Comp A') (s: list A),
+        {{ [[`vret <~~ acc as _]] :: [[`vhead <-- head as _]] :: tenv }}
+          facadeBody
+        {{ [[`vret <~~ (f acc head) as _]] :: tenv }} ∪
+        {{ [vtest <-- wrap (bool2w false)] :: [vlst <-- wrap s] :: ext }} // env) ->
+    {{ [[`vret <~~ init as _]] :: [[`vlst <-- lst as _]] :: tenv }}
+      (Seq (Fold vhead vtest vlst fpop fempty facadeBody) (Call (DummyArgument vtest) fdealloc (vlst :: nil)))
+    {{ [[`vret <~~ (fold_left f lst init) as _]] :: tenv }} ∪ {{ ext }} // env.
+Proof.
+  unfold DummyArgument; loop_t.
+
+  rewrite TelEq_swap by loop_t;
+    eapply CompileCallEmpty_spec; loop_t.
+
+  2:eapply CompileCallFacadeImplementationOfDestructor; loop_t.
+
+  loop_unify_with_nil_t.
+
+  loop_t.
+  generalize dependent init;
+  induction lst; loop_t.
+
+  move_to_front vtest;
+  apply CompileWhileFalse_Loop; loop_t.
+
+  eapply CompileWhileTrue; [ loop_t.. | ].
+
+  apply generalized @CompileCallPop; loop_t.
+
+  move_to_front vlst; apply ProgOk_Chomp_Some; loop_t.
+  move_to_front vtest; apply ProgOk_Chomp_Some; loop_t.
+  computes_to_inv; subst; defunctionalize_evar; eauto.
+
+  rewrite TelEq_swap; eauto.
+  apply CompileCallEmpty_spec; loop_t.
+
+  loop_t.
+Qed.
+
+Lemma CompileLoop :
+  forall `{FacadeWrapper (Value av) A} `{FacadeWrapper (Value av) A'} `{FacadeWrapper av (list A)}
+    lst init vhead vtest vlst vret fpop fempty fdealloc facadeBody facadeConclude
+    env (ext: StringMap.t (Value av)) tenv tenv' (f: Comp A' -> A -> Comp A'),
+    GLabelMap.MapsTo fpop (Axiomatic (List_pop A)) env ->
+    GLabelMap.MapsTo fempty (Axiomatic (List_empty A)) env ->
+    GLabelMap.MapsTo fdealloc (Axiomatic (FacadeImplementationOfDestructor (list A))) env ->
+    PreconditionSet tenv ext [[[vhead; vtest; vlst; vret]]] ->
+    {{ [[`vret <~~ (fold_left f lst init) as _]] :: tenv }}
+      facadeConclude
+    {{ [[`vret <~~ (fold_left f lst init) as _]] :: tenv' }} ∪ {{ ext }} // env ->
+    (forall head (acc: Comp A') (s: list A),
+        {{ [[`vret <~~ acc as _]] :: [[`vhead <-- head as _]] :: tenv }}
+          facadeBody
+        {{ [[`vret <~~ (f acc head) as _]] :: tenv }} ∪
+        {{ [vtest <-- wrap (bool2w false)] :: [vlst <-- wrap s] :: ext }} // env) ->
+    {{ [[`vret <~~ init as _]] :: [[`vlst <-- lst as _]] :: tenv }}
+      (Seq (Seq (Fold vhead vtest vlst fpop fempty facadeBody) (Call (DummyArgument vtest) fdealloc (vlst :: nil))) facadeConclude)
+    {{ [[`vret <~~ (fold_left f lst init) as _]] :: tenv' }} ∪ {{ ext }} // env.
+Proof.
+  eauto using @CompileSeq, @CompileLoopBase.
+Qed.
+
+Lemma CompileLoopAlloc :
+  forall `{FacadeWrapper (Value av) A} `{FacadeWrapper (Value av) A'} `{FacadeWrapper av (list A)}
+    lst init vhead vtest vlst vret fpop fempty fdealloc facadeInit facadeBody facadeConclude
+    env (ext: StringMap.t (Value av)) tenv tenv' (f: Comp A' -> A -> Comp A'),
+    GLabelMap.MapsTo fpop (Axiomatic (List_pop A)) env ->
+    GLabelMap.MapsTo fempty (Axiomatic (List_empty A)) env ->
+    GLabelMap.MapsTo fdealloc (Axiomatic (FacadeImplementationOfDestructor (list A))) env ->
+    PreconditionSet tenv ext [[[vhead; vtest; vlst; vret]]] ->
+    {{ [[`vlst <-- lst as _]] :: tenv }}
+      facadeInit
+    {{ [[`vret <~~ init as _]] :: [[`vlst <-- lst as _]] :: tenv }} ∪ {{ ext }} // env ->
+    {{ [[`vret <~~ (fold_left f lst init) as _]] :: tenv }}
+      facadeConclude
+    {{ [[`vret <~~ (fold_left f lst init) as _]] :: tenv' }} ∪ {{ ext }} // env ->
+    (forall head (acc: Comp A') (s: list A),
+        {{ [[`vret <~~ acc as _]] :: [[`vhead <-- head as _]] :: tenv }}
+          facadeBody
+        {{ [[`vret <~~ (f acc head) as _]] :: tenv }} ∪
+        {{ [vtest <-- wrap (bool2w false)] :: [vlst <-- wrap s] :: ext }} // env) ->
+    {{ [[`vlst <-- lst as _]] :: tenv }}
+      (Seq facadeInit (Seq (Seq (Fold vhead vtest vlst fpop fempty facadeBody) (Call (DummyArgument vtest) fdealloc (vlst :: nil))) facadeConclude))
+    {{ [[`vret <~~ (fold_left f lst init) as _]] :: tenv' }} ∪ {{ ext }} // env.
+Proof.
+  eauto using @CompileSeq, @CompileLoop.
+Qed.
+
+Definition revmap {A B} f := fun seq => @map A B f (rev seq).
+
+Lemma revmap_fold_helper:
+  forall (A A' : Type) (f : A -> A') (a : A) (vv : list A) (base : list A'),
+    revmap f (a :: vv) ++ base = revmap f vv ++ f a :: base.
+Proof.
+  unfold revmap; intros; simpl.
+  rewrite map_rev.
+  rewrite map_app.
+  simpl.
+  rewrite <- app_assoc.
+  simpl.
+  rewrite <- map_rev.
+  reflexivity.
+Qed.
+
+Lemma revmap_fold_generalized :
+  forall {A B} (f: A -> B) (seq: list A) (base: list B),
+    fold_left (fun acc elem => f elem :: acc) seq base = (@revmap A B f seq) ++ base.
+Proof.
+  induction seq; simpl; intros.
+  - reflexivity.
+  - rewrite revmap_fold_helper; eauto.
+Qed.
+
+Lemma revmap_fold :
+  forall {A B} (f: A -> B) (seq: list A),
+    fold_left (fun acc elem => f elem :: acc) seq nil = @revmap A B f seq.
+Proof.
+  intros.
+  rewrite <- (app_nil_r (revmap f seq)).
+  apply revmap_fold_generalized.
+Qed.
+
+Lemma revmap_fold_comp_generalized :
+  forall {A B} (f: A -> B) (seq: list A) base,
+    Monad.equiv
+      (fold_left (fun cacc elem => (acc <- cacc; ret (f elem :: acc))%comp) seq base)
+      ( b <- base;
+        ret ((@revmap A B f seq) ++ b)).
+Proof.
+  intros; etransitivity.
+  2: apply Monad.computes_under_bind; intros; rewrite <- revmap_fold_generalized; apply SetoidMorphisms.equiv_refl.
+
+  generalize dependent base; induction seq; simpl;
+  [ | setoid_rewrite IHseq ];
+  split; intros; computes_to_inv; subst; eauto using BindComputes.
+Qed.
+
+Lemma revmap_fold_comp :
+  forall {A B} (f: A -> B) (seq: list A),
+    Monad.equiv
+      (fold_left (fun cacc elem => (acc <- cacc; ret (f elem :: acc))%comp) seq (ret nil))
+      (ret (@revmap A B f seq)).
+Proof.
+  intros.
+  rewrite <- (app_nil_r (revmap f seq)).
+  rewrite revmap_fold_comp_generalized.
+  split; intros; computes_to_inv; subst; eauto using BindComputes.
+Qed.
+
+Lemma CompileMapAlloc_ADT :
+  forall {av A A'} `{FacadeWrapper av (list A)} `{FacadeWrapper av (list A')} `{FacadeWrapper (Value av) A} `{FacadeWrapper av A'}
+    (lst: list A) vhead vhead' vtest vlst vret vtmp fpop fempty falloc fdealloc fcons facadeBody facadeCoda env (ext: StringMap.t (Value av)) tenv tenv' (f: A -> A'),
+    GLabelMap.MapsTo fpop (Axiomatic (List_pop A)) env ->
+    GLabelMap.MapsTo fempty (Axiomatic (List_empty A)) env ->
+    GLabelMap.MapsTo falloc (Axiomatic (FacadeImplementationOfConstructor (list A') nil)) env ->
+    GLabelMap.MapsTo fdealloc (Axiomatic (FacadeImplementationOfDestructor (list A))) env ->
+    GLabelMap.MapsTo fcons (Axiomatic (FacadeImplementationOfMutation_ADT A' (list A') cons)) env ->
+    (* GLabelMap.MapsTo fdealloc_one (Axiomatic (FacadeImplementationOfDestructor A)) env -> *)
+    PreconditionSet tenv ext [[[vhead; vhead'; vtest; vlst; vret; vtmp]]] ->
+    {{ [[`vret <-- (revmap f lst) as _]] :: tenv }}
+      facadeCoda
+    {{ [[`vret <-- (revmap f lst) as _]] :: tenv' }} ∪ {{ ext }} // env ->
+    (forall head (s: list A) (s': list A'),
+        {{ [[`vhead <-- head as _]] :: tenv }}
+          facadeBody
+        {{ [[`vhead' <-- f head as _]] :: tenv }} ∪
+        {{ [vret <-- wrap s'] :: [vtest <-- wrap (bool2w false)] :: [vlst <-- wrap s] :: ext }} // env) ->
+    {{ [[`vlst <-- lst as _]] :: tenv }}
+      (Seq
+         (Call vret falloc nil)
+         (Seq
+            (Seq
+               (Fold vhead vtest vlst fpop fempty
+                     (Seq facadeBody
+                          (Call vtmp fcons (vret :: vhead' :: nil))))
+               (Call vtest fdealloc (vlst :: nil)))
+            facadeCoda))
+    {{ [[`vret <-- (revmap f lst) as _]] :: tenv' }} ∪ {{ ext }} // env.
+Proof.
+  intros.
+  setoid_rewrite <- revmap_fold_comp.
+  apply CompileLoopAlloc; eauto.
+  PreconditionSet_t; eauto.
+  eapply (CompileCallFacadeImplementationOfConstructor (A := list A')); loop_t.
+  setoid_rewrite revmap_fold_comp; eassumption.
+  intros.
+  rewrite SameValues_Fiat_Bind_TelEq.
+  move_to_front vret.
+  apply miniChomp'; intros.
+  hoare.
+  apply ProgOk_Chomp_Some; loop_t; defunctionalize_evar; eauto.
+  apply CompileCallFacadeImplementationOfMutation_ADT; compile_do_side_conditions.
+Qed.
+
+Lemma CompileMapAlloc_SCA :
+  forall {av A} `{FacadeWrapper av (list A)} `{FacadeWrapper av (list W)} `{FacadeWrapper (Value av) A}
+    (lst: list A) vhead vhead' vtest vlst vret vtmp fpop fempty falloc fdealloc fcons facadeBody facadeCoda env (ext: StringMap.t (Value av)) tenv tenv' (f: A -> W),
+    GLabelMap.MapsTo fpop (Axiomatic (List_pop A)) env ->
+    GLabelMap.MapsTo fempty (Axiomatic (List_empty A)) env ->
+    GLabelMap.MapsTo falloc (Axiomatic (FacadeImplementationOfConstructor (list W) nil)) env ->
+    GLabelMap.MapsTo fdealloc (Axiomatic (FacadeImplementationOfDestructor (list A))) env ->
+    GLabelMap.MapsTo fcons (Axiomatic (FacadeImplementationOfMutation_SCA (list W) cons)) env ->
+    (* GLabelMap.MapsTo fdealloc_one (Axiomatic (FacadeImplementationOfDestructor A)) env -> *)
+    PreconditionSet tenv ext [[[vhead; vhead'; vtest; vlst; vret; vtmp]]] ->
+    {{ [[`vret <-- (revmap f lst) as _]] :: tenv }}
+      facadeCoda
+    {{ [[`vret <-- (revmap f lst) as _]] :: tenv' }} ∪ {{ ext }} // env ->
+    (forall head (s: list A) (s': list W),
+        {{ [[`vhead <-- head as _]] :: tenv }}
+          facadeBody
+        {{ [[`vhead' <-- f head as _]] :: tenv }} ∪
+        {{ [vret <-- wrap s'] :: [vtest <-- wrap (bool2w false)] :: [vlst <-- wrap s] :: ext }} // env) ->
+    {{ [[`vlst <-- lst as _]] :: tenv }}
+      (Seq
+         (Call vret falloc nil)
+         (Seq
+            (Seq
+               (Fold vhead vtest vlst fpop fempty
+                     (Seq facadeBody
+                          (Call vtmp fcons (vret :: vhead' :: nil))))
+               (Call vtest fdealloc (vlst :: nil)))
+            facadeCoda))
+    {{ [[`vret <-- (revmap f lst) as _]] :: tenv' }} ∪ {{ ext }} // env.
+Proof.
+  intros.
+  setoid_rewrite <- revmap_fold_comp.
+  apply CompileLoopAlloc; eauto.
+  PreconditionSet_t; eauto.
+  eapply (CompileCallFacadeImplementationOfConstructor (A := list W)); loop_t.
+  setoid_rewrite revmap_fold_comp; eassumption.
+  intros.
+  rewrite SameValues_Fiat_Bind_TelEq.
+  move_to_front vret.
+  apply miniChomp'; intros.
+  hoare.
+  apply ProgOk_Chomp_Some; loop_t; defunctionalize_evar; eauto.
+  apply CompileCallFacadeImplementationOfMutation_SCA; unfold DummyArgument; compile_do_side_conditions.
+Qed.
+
+Lemma ret_fold_fold_ret_lemma :
+  forall {TElem TAcc} (f: TAcc -> TElem -> TAcc) lst (init: TAcc) init_comp,
+    Monad.equiv (ret init) init_comp ->
+    Monad.equiv (ret (fold_left f lst init))
+                (fold_left (fun (acc: Comp TAcc) x => (a <- acc; ret (f a x))%comp) lst init_comp).
+Proof.
+  induction lst; simpl; intros.
+  - trivial.
+  - etransitivity; [ apply IHlst | reflexivity ].
+    unfold Monad.equiv in *; repeat (cleanup_pure || computes_to_inv || subst).
+    + eapply BindComputes; try rewrite <- H; apply ReturnComputes.
+    + rewrite <- H in *; computes_to_inv; subst; apply ReturnComputes.
+Qed.
+
+Lemma ret_fold_fold_ret :
+  forall {TElem TAcc} (f: TAcc -> TElem -> TAcc) lst (init: TAcc),
+    Monad.equiv (ret (fold_left f lst init))
+                (fold_left (fun (acc: Comp TAcc) x => (a <- acc; ret (f a x))%comp) lst (ret init)).
+Proof.
+  intros; apply ret_fold_fold_ret_lemma; apply SetoidMorphisms.equiv_refl.
+Qed.
+
+Lemma CompileLoop_ret :
+  forall {av A} `{FacadeWrapper (Value av) A} `{FacadeWrapper (Value av) A'} `{FacadeWrapper av (list A)}
+    lst init facadeBody facadeConclude vhead vtest vlst vret env (ext: StringMap.t (Value av)) tenv tenv' fpop fempty fdealloc (f: A' -> A -> A'),
+    GLabelMap.MapsTo fpop (Axiomatic (List_pop A)) env ->
+    GLabelMap.MapsTo fempty (Axiomatic (List_empty A)) env ->
+    GLabelMap.MapsTo fdealloc (Axiomatic (FacadeImplementationOfDestructor (list A))) env ->
+    PreconditionSet tenv ext [[[vhead; vtest; vlst; vret]]] ->
+    (forall head acc (s: list A),
+        {{ [[`vret <-- acc as _]] :: [[`vhead <-- head as _]] :: tenv }}
+          facadeBody
+        {{ [[`vret <-- (f acc head) as _]] :: tenv }} ∪ {{ [vtest <-- wrap (bool2w false)] :: [vlst <-- wrap s] :: ext }} // env) ->
+    {{ [[`vret <-- (fold_left f lst init) as _]] :: tenv }}
+      facadeConclude
+    {{ [[`vret <-- (fold_left f lst init) as _]] :: tenv' }} ∪ {{ ext }} // env ->
+    {{ [[`vret <-- init as _]] :: [[`vlst <-- lst as _]] :: tenv }}
+      (Seq (Seq (Fold vhead vtest vlst fpop fempty facadeBody) (Call (DummyArgument vtest) fdealloc (vlst :: nil))) facadeConclude)
+    {{ [[`vret <-- (fold_left f lst init) as _]] :: tenv' }} ∪ {{ ext }} // env.
+Proof.
+  intros.
+  setoid_rewrite ret_fold_fold_ret.
+  eapply CompileSeq.
+  apply CompileLoopBase; eauto.
+  2: apply ProkOk_specialize_to_ret; intros * h; apply ret_fold_fold_ret in h; computes_to_inv; subst; eauto.
+  intros; rewrite SameValues_Fiat_Bind_TelEq.
+  apply miniChomp'; intros; eauto.
+Qed.
+
+Lemma CompileLoopAlloc_ret :
+  forall {av A} `{FacadeWrapper (Value av) A} `{FacadeWrapper (Value av) A'} `{FacadeWrapper av (list A)}
+    lst init facadeInit facadeBody facadeConclude vhead vtest vlst vret env (ext: StringMap.t (Value av)) tenv tenv' fpop fempty fdealloc (f: A' -> A -> A'),
+    GLabelMap.MapsTo fpop (Axiomatic (List_pop A)) env ->
+    GLabelMap.MapsTo fempty (Axiomatic (List_empty A)) env ->
+    GLabelMap.MapsTo fdealloc (Axiomatic (FacadeImplementationOfDestructor (list A))) env ->
+    PreconditionSet tenv ext [[[vhead; vtest; vlst; vret]]] ->
+    {{ [[`vlst <-- lst as _]] :: tenv }}
+      facadeInit
+    {{ [[`vret <-- init as _]] :: [[`vlst <-- lst as _]] :: tenv }} ∪ {{ ext }} // env ->
+    (forall head acc (s: list A),
+        {{ [[`vret <-- acc as _]] :: [[`vhead <-- head as _]] :: tenv }}
+          facadeBody
+        {{ [[`vret <-- (f acc head) as _]] :: tenv }} ∪ {{ [vtest <-- wrap (bool2w false)] :: [vlst <-- wrap s] :: ext }} // env) ->
+    {{ [[`vret <-- (fold_left f lst init) as _]] :: tenv }}
+      facadeConclude
+    {{ [[`vret <-- (fold_left f lst init) as _]] :: tenv' }} ∪ {{ ext }} // env ->
+    {{ [[`vlst <-- lst as _]] :: tenv }}
+      (Seq facadeInit (Seq (Seq (Fold vhead vtest vlst fpop fempty facadeBody) (Call (DummyArgument vtest) fdealloc (vlst :: nil))) facadeConclude))
+    {{ [[`vret <-- (fold_left f lst init) as _]] :: tenv' }} ∪ {{ ext }} // env.
+Proof.
+  eauto using @CompileSeq, @CompileLoop_ret.
+Qed.
+
+
+Lemma SameValues_Fiat_Bind_TelEq_Pair :
+  forall {av A1 A2 B} key compA compB tail ext,
+    TelEq ext
+          (Cons (av := av) key (@Bind (A1 * A2) B compA compB) tail)
+          (Cons NTNone compA (fun a => Cons NTNone (ret (fst a)) (fun a1 => Cons NTNone (ret (snd a)) (fun a2 => Cons key (compB (a1, a2)) tail)))).
+Proof.
+  unfold TelEq;
+  repeat match goal with
+         | _ => progress subst
+         | _ => progress SameValues_Fiat_t_step
+         | _ => rewrite <- surjective_pairing in *
+         end.
+Qed.
+
+Lemma ProgOk_Transitivity_Name_Pair :
+  forall {av A1 A2} `{FacadeWrapper av A1} `{FacadeWrapper av A2} {ext env}
+    vfst vsnd tenv tenv' (pair: Comp (A1 * A2)) prog d1 d2,
+    {{ tenv }}
+      prog
+    {{ [[pair as p]] :: [[`vfst <-- fst p as p1]] :: [[`vsnd <-- snd p as p2]] :: tenv' p1 p2 }} ∪ {{ext}} // env ->
+    {{ [[pair as p]] :: [[`vfst <-- fst p as p1]] :: [[`vsnd <-- snd p as p2]] :: tenv' p1 p2 }}
+      d1
+    {{ [[pair as p]] :: [[ret (fst p) as p1]] :: [[`vsnd <-- snd p as p2]] :: tenv' p1 p2 }} ∪ {{ext}} // env ->
+    {{ [[pair as p]] :: [[ret (fst p) as p1]] :: [[`vsnd <-- snd p as p2]] :: tenv' p1 p2 }}
+      d2
+    {{ [[pair as p]] :: [[ret (fst p) as p1]] :: [[ret (snd p) as p2]] :: tenv' p1 p2 }} ∪ {{ext}} // env ->
+    {{ tenv }}
+      Seq prog (Seq d1 d2)
+    {{ [[pair as p]] :: [[ret (fst p) as p1]] :: [[ret (snd p) as p2]] :: tenv' p1 p2 }} ∪ {{ext}} // env.
+Proof.
+  repeat hoare.
+Qed.
+
+Lemma CompileDeallocADT_discretely : (* TODO create a specialized version that hardcodes the deallocation call *)
+  forall {av A} {env ext} (k: NameTag av A) comp tenv tenv' prog dealloc,
+    {{ [[k <~~ comp as kk]] :: tenv kk }}
+      prog
+      {{ [[k <~~ comp as kk]] :: tenv' kk }} ∪ {{ext}} // env ->
+    {{ [[k <~~ comp as kk]] :: tenv' kk }}
+      dealloc
+      {{ [[comp as kk]] :: tenv' kk }} ∪ {{ext}} // env ->
+    {{ [[k <~~ comp as kk]] :: tenv kk }}
+      (Seq prog dealloc)
+      {{ [[comp as kk]] :: tenv' kk }} ∪ {{ext}} // env.
+Proof.
+  repeat hoare.
+Qed.
+
+Lemma CompileDeallocADT_discretely' : (* TODO create a specialized version that hardcodes the deallocation call *)
+  forall {av A} {env ext} (k: NameTag av A) v tenv tenv' prog dealloc,
+    {{ [[k <-- v as _]] :: tenv }}
+      prog
+    {{ [[k <-- v as _]] :: tenv' }} ∪ {{ext}} // env ->
+    {{ [[k <-- v as _]] :: tenv' }}
+      dealloc
+    {{ tenv' }} ∪ {{ext}} // env ->
+    {{ [[k <-- v as _]] :: tenv }}
+      (Seq prog dealloc)
+    {{ tenv' }} ∪ {{ext}} // env.
+Proof.
+  repeat hoare.
+Qed.
+
+  Ltac facade_if_helper ::=     (* Add an eauto 3 to prevent spurious existentials from popping up *)
+  match goal with
+  | H:is_true ?st (isTrueExpr ?k),
+    H':StringMap.MapsTo ?k (wrap (bool2w ?test)) ?st
+    |- _ => learn (is_true_isTrueExpr H H')
+  | H:is_false ?st (isTrueExpr ?k),
+    H':StringMap.MapsTo ?k (wrap (bool2w ?test)) ?st
+    |- _ => learn (is_false_isTrueExpr H H')
+  | _ => solve
+  [ eauto 3 using isTrueExpr_is_false, isTrueExpr_is_true  with SameValues_db ]
+  | _ => solve
+  [ eauto using isTrueExpr_is_false, isTrueExpr_is_true  with SameValues_db ]
+  end.
+
+Lemma CompileIf :
+  forall {av A} k tmp (gallinaTest: bool) (gallinaT gallinaF: Comp A) facadeTest facadeT facadeF
+    env (ext: StringMap.t (Value av)) tenv tenv',
+    tmp ∉ ext ->
+    NotInTelescope tmp tenv ->
+    {{ tenv }}
+      facadeTest
+    {{ [[`tmp <-- (bool2w gallinaTest) as _]]::tenv }} ∪ {{ ext }} // env ->
+    {{ [[`tmp <-- (bool2w gallinaTest) as _]]::tenv }}
+      facadeT
+    {{ [[`tmp <-- (bool2w gallinaTest) as _]]::[[k <~~ gallinaT as v]]::tenv' v }} ∪ {{ ext }} // env ->
+    {{ [[`tmp <-- (bool2w gallinaTest) as _]]::tenv }}
+      facadeF
+    {{ [[`tmp <-- (bool2w gallinaTest) as _]]::[[k <~~ gallinaF as v]]::tenv' v }} ∪ {{ ext }} // env ->
+    {{ tenv }}
+      (Seq facadeTest (DFacade.If (isTrueExpr tmp) facadeT facadeF))
+    {{ [[k <~~ if gallinaTest then gallinaT else gallinaF as v]]::tenv' v }} ∪ {{ ext }} // env.
+Proof.
+  intros; hoare.
+  repeat (SameValues_Facade_t_step || facade_if_helper).
+Qed.
+
+(* FIXME move stuff above to Extraction.Extraction *)
+
+
+Lemma SameValues_remove_SCA:
+  forall (av0 : Type) (tenv' : Telescope av0)
+    (ext : StringMap.t (Value av0)) (k : StringMap.key)
+    (final_state : State av0) (x : W),
+    StringMap.MapsTo k (wrap x) final_state ->
+    StringMap.remove (elt:=Value av0) k final_state ≲ tenv' ∪ ext ->
+    final_state ≲ tenv' ∪ ext.
+Proof.
+  induction tenv'; simpl; intros.
+  - rewrite (add_redundant_cancel H).
+    rewrite <- add_remove_cancel; try reflexivity.
+    apply WeakEq_pop_SCA.
+    apply StringMap.remove_1; reflexivity.
+    assumption.
+  - destruct key; repeat cleanup.
+    + eauto.
+    + SameValues_Fiat_t.
+      StringMap_t.
+      rewrite remove_mapsto_iff in *.
+      cleanup.
+      StringMap_t.
+      repeat cleanup.
+      eapply H.
+      2: rewrite remove_remove_comm; eauto.
+      rewrite remove_mapsto_iff in *; eauto.
+Qed.
+
+Hint Resolve SameValues_remove_SCA : SameValues_db.
+
+Lemma CompileDeallocSCA_discretely :
+  forall {av} (tenv tenv': Telescope av) ext env k (v: Comp W) prog,
+    k ∉ ext ->
+    NotInTelescope k tenv ->
+    {{ [[`k <~~ v as _]] :: tenv }} prog {{ [[`k <~~ v as _]] :: tenv' }} ∪ {{ ext }} // env ->
+    {{ [[`k <~~ v as _]] :: tenv }} prog {{ tenv' }} ∪ {{ ext }} // env.
+Proof.
+  SameValues_Facade_t.
+Qed.
+
+Lemma ProgOk_Chomp_Some_snd :
+  forall {av A T} `{FacadeWrapper (Value av) A} `{FacadeWrapper (Value av) T} env key value k (v': Comp T) prog
+    (tail1: A -> Telescope av)
+    (tail2: A -> Telescope av)
+    ext,
+    key ∉ ext ->
+    (forall v: A, value ↝ v -> {{ tail1 v }} prog {{ Cons (NTSome k) v' (fun _ => tail2 v) }} ∪ {{ [key <-- wrap v] :: ext }} // env) ->
+    ({{ Cons (NTSome key) value tail1 }} prog {{ Cons (NTSome k) v' (fun _ => Cons (NTSome key) value tail2) }} ∪ {{ ext }} // env).
+Proof.
+  intros.
+  rewrite TelEq_swap.
+  apply ProgOk_Chomp_Some; eauto.
+Qed.
+
+Lemma ProgOk_Chomp_None_snd :
+  forall {av A T} `{FacadeWrapper (Value av) T} env key value prog
+    (tail1: A -> Telescope av)
+    (tail2: A -> Telescope av)
+    ext k (v': Comp T),
+    key ∉ ext ->
+    (forall v: A, value ↝ v -> {{ tail1 v }} prog {{ Cons (NTSome k) v' (fun _ => tail2 v) }} ∪ {{ ext }} // env) ->
+    ({{ Cons NTNone value tail1 }} prog {{ Cons (NTSome k) v' (fun _ => Cons NTNone value tail2) }} ∪ {{ ext }} // env).
+Proof.
+  intros.
+  rewrite TelEq_swap.
+  apply ProgOk_Chomp_None; eauto.
+Qed.
+
+Lemma CompileCallFacadeImplementationOfMutation_ADT_Replace_strong:
+  forall {av Targ Tadt} `{FacadeWrapper av Tadt} `{FacadeWrapper av Targ} {env} fADT,
+  forall fpointer varg vtmp (arg: Targ) (target: Tadt) tenv tenv',
+    GLabelMap.MapsTo fpointer (Axiomatic (FacadeImplementationOfMutation_ADT Targ Tadt fADT)) env ->
+    forall vret ext pArg pCoda,
+      PreconditionSet tenv ext [[[varg; vtmp; vret]]] ->
+      {{ [[ `vret <-- target as _]] :: tenv }}
+        pArg
+        {{ [[ `vret <-- target as _]] :: [[ `varg <-- arg as _]] :: tenv }} ∪ {{ ext }} // env ->
+      {{ [[ `vret <-- (fADT arg target) as _]] :: tenv }}
+        pCoda
+        {{ [[ `vret <-- (fADT arg target) as _]] :: tenv' }} ∪ {{ ext }} // env ->
+      {{ [[ `vret <-- target as _]] :: tenv }}
+        Seq (Seq pArg (Call vtmp fpointer (vret :: varg :: nil))) pCoda
+        {{ [[ `vret <-- (fADT arg target) as _]] :: tenv' }} ∪ {{ ext }} // env.
+Proof.
+  intros; hoare.
+  apply CompileCallFacadeImplementationOfMutation_ADT_Replace; PreconditionSet_t; eauto.
+Qed.
+
+Lemma CompileCallFacadeImplementationOfMutation_SCA_Replace_strong:
+  forall {av Tadt} `{FacadeWrapper av Tadt} {env} fADT,
+  forall fpointer varg vtmp (arg: W) (target: Tadt) tenv tenv',
+    GLabelMap.MapsTo fpointer (Axiomatic (FacadeImplementationOfMutation_SCA Tadt fADT)) env ->
+    forall vret ext pArg pCoda,
+      PreconditionSet tenv ext [[[varg; vtmp; vret]]] ->
+      {{ [[ `vret <-- target as _]] :: tenv }}
+        pArg
+        {{ [[ `vret <-- target as _]] :: [[ `varg <-- arg as _]] :: tenv }} ∪ {{ ext }} // env ->
+      {{ [[ `vret <-- (fADT arg target) as _]] :: tenv }}
+        pCoda
+        {{ [[ `vret <-- (fADT arg target) as _]] :: tenv' }} ∪ {{ ext }} // env ->
+      {{ [[ `vret <-- target as _]] :: tenv }}
+        Seq (Seq pArg (Call vtmp fpointer (vret :: varg :: nil))) pCoda
+        {{ [[ `vret <-- (fADT arg target) as _]] :: tenv' }} ∪ {{ ext }} // env.
+Proof.
+  intros; hoare.
+  apply CompileCallFacadeImplementationOfMutation_SCA_Replace; PreconditionSet_t; eauto.
+Qed.
+
+(* FIXME rename ProkOk_specialize_to_ret *)
+(* FIXME Move stuff above *)
+
+(* Ltac compile_chomp := *)
+(*   match_ProgOk *)
+(*     ltac:(fun prog pre post ext env => *)
+(*             match pre with    (* FIXME could be generalized beyond the first binding *) *)
+(*             | Cons ?k ?v ?tenv => *)
+(*               match post with *)
+(*               | Cons k v _ => fail 1 *)
+(*               | context[Cons k v _] => move_to_front k *)
+(*               end *)
+(*             end). *)
+
+Ltac _compile_map :=
+  match_ProgOk
+    ltac:(fun prog pre post ext env =>
+            let vhead := gensym "head" in
+            let vhead' := gensym "head'" in
+            let vtest := gensym "test" in
+            let vtmp := gensym "tmp" in
+            match constr:(pre, post) with
+            | (Cons (NTSome ?vseq) (ret ?seq) ?tenv, Cons (NTSome ?vret) (ret (revmap _ ?seq')) ?tenv') =>
+              unify seq seq';
+                first [
+                    apply (CompileMapAlloc_SCA seq (vhead := vhead) (vhead' := vhead') (vtest := vtest) (vtmp := DummyArgument vtmp)) |
+                    apply (CompileMapAlloc_ADT seq (vhead := vhead) (vhead' := vhead') (vtest := vtest) (vtmp := DummyArgument vtmp)) ]
+            end).
+
+Ltac _compile_chomp :=         (* This is a weak version of the real compile_chomp, which is too slow *)
+  match_ProgOk
+    ltac:(fun prog pre post ext env =>
+            match constr:(pre, post) with
+            | (Cons ?k ?v ?tenv, Cons ?k' ?v' ?tenv') =>
+              unify k k'; unify v v';
+              match k with
+              | NTNone => apply ProgOk_Chomp_None
+              | _ => apply ProgOk_Chomp_Some
+              end
+            | (Cons ?k ?v ?tenv, Cons _ _ (fun _ => Cons ?k' ?v' ?tenv')) =>
+              unify k k'; unify v v';
+              match k with
+              | NTNone => apply ProgOk_Chomp_None_snd
+              | _ => apply ProgOk_Chomp_Some_snd
+              end
+            end).
+
+Ltac tenv_mentions env v :=
+  first [ match env with
+          | context[?vv] => first [ is_evar vv; fail 1
+                                 | unify v vv; fail 2 ]
+          | _ => idtac
+          end; fail 1 | idtac ].
+
+Ltac tenv_mentions_fast env v :=
+  lazymatch v with
+  | ?f => match env with context[f] => idtac end
+  | ?f ?a => match env with context[f ?a'] => unify a a' end
+  | ?f ?a ?b => match env with context[f ?a' ?b'] => unify a a'; unify b b' end
+  | ?f ?a ?b ?c => match env with context[f ?a' ?b' ?c'] => unify a a'; unify b b'; unify c c' end
+  | ?f ?a ?b ?c ?d => match env with context[f ?a' ?b' ?c' ?d'] => unify a a'; unify b b'; unify c c'; unify d d' end
+  end.
+
+Ltac _compile_destructor_unsafe vtmp tenv tenv' :=
+  (apply CompileDeallocSCA_discretely ||
+   first [ unify tenv tenv';
+           apply (CompileCallFacadeImplementationOfDestructor (vtmp := DummyArgument vtmp))
+         | eapply CompileSeq;
+           [ apply (CompileCallFacadeImplementationOfDestructor (vtmp := DummyArgument vtmp)) | ] ]);
+  try compile_do_side_conditions.
+
+Ltac _compile_destructor :=
+  match_ProgOk
+     ltac:(fun prog pre post ext env =>
+             let vtmp := gensym "tmp" in
+             match pre with
+             | Cons _ ?v (fun _ => ?tenv) =>
+               match tenv with
+               | context[post] => _compile_destructor_unsafe vtmp tenv post
+               | _ => unify tenv post; _compile_destructor_unsafe vtmp tenv post
+               | _ => lazymatch v with
+                 | ret ?vv => first [ tenv_mentions_fast post vv; fail 1
+                                   | _compile_destructor_unsafe vtmp tenv post ]
+                 | ?vv => first [ tenv_mentions_fast post vv; fail 1
+                               | _compile_destructor_unsafe vtmp tenv post ]
+                 end
+               end
+             end).
+
+Ltac unifiable t1 t2 :=
+  match constr:(true) with
+  | _ => let pr := constr:(eq_refl t1 : t1 = t2) in
+        constr:true
+  | _ => constr:false
+  end.
+
+Ltac is_sca_comp v :=
+  match type of v with
+  | Comp ?w => let r := unifiable w W in constr:r
+  end.
+
+Ltac _compile_destructor ::=
+    match_ProgOk
+      ltac:(fun prog pre post ext env =>
+              let vtmp := gensym "tmp" in
+              match pre with
+              | Cons (NTSome ?k) ?v (fun _ => ?tenv) =>
+                match tenv with
+                | context[post] => (* post is a suffix of pre *)
+                  _compile_destructor_unsafe vtmp tenv post
+                | _ => (* post is pre *)
+                  unify tenv post; _compile_destructor_unsafe vtmp tenv post
+                | _ => let is_sca := is_sca_comp v in
+                      lazymatch is_sca with
+                      | true => (match post with
+                                | context[k] => fail 1
+                                | _ => apply CompileDeallocSCA_discretely
+                                end)
+                      | false => (lazymatch v with
+                                  | ret ?vv => first [ tenv_mentions_fast post vv; fail 1
+                                                    | _compile_destructor_unsafe vtmp tenv post ]
+                                  | ?vv => first [ tenv_mentions_fast post vv; fail 1
+                                                | _compile_destructor_unsafe vtmp tenv post ]
+                                  end)
+                      end
+                end
+              end).
+
+Ltac _compile_skip :=
+  match_ProgOk
+    ltac:(fun prog pre post ext env =>
+            match constr:(pre, post) with
+            | (?tenv, ?tenv') => not_evar tenv; not_evar tenv'; unify tenv tenv'; apply CompileSkip
+            end).
+
+Ltac _compile_if :=
+  match_ProgOk
+    ltac:(fun prog pre post ext env =>
+            match constr:(pre, post) with
+            | (_, Cons _ (if _ then _ else _) _) =>
+              let vtest := gensym "test" in
+              apply (CompileIf (tmp := vtest))
+            end).
+
+Ltac __compile_prepare_chomp tenv tenv' :=
+  match tenv with
+  | Cons ?k ?v _ =>
+    match tenv' with
+    | Cons ?k' ?v' _ =>
+      unify k k'; unify v v';
+      fail 1 (* Nothing to do: can already chomp *)
+    | Cons _ _ (fun _ => ?tail) =>
+      unify tenv tail; idtac;
+      fail 1 (* This is a job for deallocation, not chomping *)
+    | context[Cons k v _] =>
+      move_to_front k
+    end
+  end.
+
+Ltac _compile_prepare_chomp :=
+  match_ProgOk
+    ltac:(fun prog pre post ext env =>
+            is_evar prog;
+            first [ __compile_prepare_chomp pre post
+                  | __compile_prepare_chomp post pre ]).
+
+Ltac useless_binder term :=
+  lazymatch term with
+  | (fun _ => ?body) => let capture := body in idtac
+  end.
+
+Ltac _compile_rewrite_bind :=
+  (* setoid_rewrite at the speed of light *)
+  match_ProgOk
+    ltac:(fun prog pre post ext env =>
+            match constr:(pre, post) with
+            | context[Cons ?k (ret _) ?tail] =>
+              first [ useless_binder tail; fail 1 |
+                      match k with
+                      | NTSome _ => setoid_rewrite Propagate_ret
+                      | NTNone => setoid_rewrite Propagate_anonymous_ret
+                      end ]
+            | context[Cons _ (Bind _ _) _] => setoid_rewrite SameValues_Fiat_Bind_TelEq
+            end).
+
+Ltac first_arg f :=
+  match type of f with
+  | ?a -> _ => a
+  end.
+
+Ltac _compile_mutation :=
+  match_ProgOk
+    ltac:(fun prog pre post ext env =>
+            match post with
+            | [[`?s <-- ?f _ _ as _]]::?tenv =>
+              let arg := gensym "arg" in
+              let tmp := gensym "tmp" in
+              let fst := first_arg f in
+              let uses_sca := unifiable fst W in
+              lazymatch uses_sca with
+              | true => match pre with
+                       | context[Cons (NTSome s) _ _] =>
+                         move_to_front s;
+                           first [ eapply (CompileCallFacadeImplementationOfMutation_SCA (vtmp:=DummyArgument tmp))
+                                 | eapply (CompileCallFacadeImplementationOfMutation_SCA_Replace (varg:=arg) (vtmp:=DummyArgument tmp))
+                                 | eapply (CompileCallFacadeImplementationOfMutation_SCA_Replace_strong (varg:=arg) (vtmp:=DummyArgument tmp))
+                                 | fail 1 ]
+                       | tenv => eapply (CompileCallFacadeImplementationOfMutation_SCA_Alloc (varg:=arg) (vtmp:=DummyArgument tmp))
+                       end
+              | false => match pre with
+                        | context[Cons (NTSome s) _ _] =>
+                          move_to_front s;
+                            first [ eapply (CompileCallFacadeImplementationOfMutation_ADT (vtmp:=DummyArgument tmp))
+                                  | eapply (CompileCallFacadeImplementationOfMutation_ADT_Replace (varg:=arg) (vtmp:=DummyArgument tmp))
+                                  | eapply (CompileCallFacadeImplementationOfMutation_ADT_Replace_strong (varg:=arg) (vtmp:=DummyArgument tmp))
+                                  | fail 1 ]
+                        | tenv => eapply (CompileCallFacadeImplementationOfMutation_ADT_Alloc (varg:=arg) (vtmp:=DummyArgument tmp))
+                        end
+              end; ensure_all_pointers_found
+            end).
+
+Ltac _compile_constructor :=
+  match_ProgOk
+    ltac:(fun prog pre post ext env =>
+            match constr:(pre, post) with
+            | (?tenv, [[?s <-- ?adt as _]]::?tenv') =>
+              match type of adt with
+              | W => fail 1
+              | _ => call_tactic_after_moving_head_binding_to_separate_goal
+                      ltac:(apply CompileCallFacadeImplementationOfConstructor);
+                  ensure_all_pointers_found
+              end
+            end).
+Ltac _compile_loop :=
+  match_ProgOk
+    ltac:(fun prog pre post ext env =>
+            let vtest := gensym "test" in
+            let vhead := gensym "head" in
+            match constr:(pre, post) with
+            | ([[`?vinit <~~ ?init as _]] :: [[`?vseq <-- ?seq as _]] :: ?tenv, [[`?vret <~~ fold_left _ ?seq ?init as _]] :: ?tenv') =>
+              apply (CompileLoop seq init (vtest := vtest) (vhead := vhead))
+            | ([[`?vinit <-- ?init as _]] :: [[`?vseq <-- ?seq as _]] :: ?tenv, [[`?vret <-- fold_left _ ?seq ?init as _]] :: ?tenv') =>
+              apply (CompileLoop_ret seq init (vtest := vtest) (vhead := vhead))
+            | ([[`?vseq <-- ?seq as _]] :: ?tenv, [[`?vret <~~ fold_left _ ?seq _ as _]] :: ?tenv') =>
+              apply (CompileLoopAlloc (vtest := vtest) (vhead := vhead))
+            | ([[`?vseq <-- ?seq as _]] :: ?tenv, [[`?vret <-- fold_left _ ?seq _ as _]] :: ?tenv') =>
+              apply (CompileLoopAlloc_ret (vtest := vtest) (vhead := vhead))
+            end).
+
+(* Ltac compile_miniChomp := *)
+(*   match_ProgOk *)
+(*     ltac:(fun prog pre post ext env => *)
+(*             match post with *)
+(*             | Cons NTNone ?v ?tenv' => *)
+(*               match pre with *)
+(*               | context[Cons ?k v _] => *)
+(*                 move_to_front k; *)
+(*                   apply miniChomp' *)
+(*               end *)
+(*             end). *)
+
+Ltac start_compiling :=
+  match goal with
+  | |- sigT _ => eexists; intros
+  end.                        (* FIXME format of progOk notation *)
+
+Ltac _compile_rewrite_if :=
+  match_ProgOk
+    ltac:(fun prog pre post ext env =>
+            match post with
+            | appcontext [if ?b then ?x else ?y] => is_dec b; setoid_rewrite (dec2bool_correct b x y)
+            | appcontext [?f (if ?b then ?x else ?y)] => is_pushable_head_constant f; setoid_rewrite (push_if f x y b)
+            end).
+
+Ltac _compile_early_hook := fail.
+Ltac _compile_late_hook := fail.
+
+Ltac _compile_step :=
+  match goal with
+  | _ => start_compiling
+  | _ => progress subst
+  | _ => progress intros
+  | _ => progress computes_to_inv
+  | _ => compile_do_side_conditions
+  | _ => _compile_early_hook
+  | _ => _compile_rewrite_bind
+  | _ => _compile_skip
+  | _ => _compile_map
+  | _ => _compile_loop
+  (* | _ => _compile_CallBagFind *)
+  (* | _ => _compile_CallBagInsert *)
+  (* | _ => _compile_CallGetAttribute *)
+  | _ => _compile_chomp
+  | _ => _compile_prepare_chomp
+  | _ => _compile_if
+  | _ => _compile_mutation
+  | _ => _compile_constructor
+  | _ => compile_simple
+  | _ => _compile_destructor
+  | _ => _compile_rewrite_if
+  | _ => _compile_late_hook
+  (* | _ => progress simpl *)
+  end.
+
+Ltac _compile :=
+  repeat _compile_step.
+
+Ltac compile_do_side_conditions_internal ::=
+  repeat cleanup; PreconditionSet_t;
+   match goal with
+   | _ => exact I
+   | |- _ <> _ => discriminate 1
+   | |- _ ∉ _ => decide_not_in
+   | |- NotInTelescope _ _ => decide_NotInTelescope
+   | |- StringMap.find _ _ = Some _ => decide_mapsto_maybe_instantiate
+   | |- StringMap.MapsTo _ _ _ => decide_mapsto_maybe_instantiate
+   | |- GLabelMap.MapsTo _ _ _ => GLabelMapUtils.decide_mapsto_maybe_instantiate
+   end.
+
+Opaque DummyArgument.
+Opaque Word.wordToNat.
+Opaque Word.natToWord.
+Opaque nat_as_constant nat_as_word string_as_var.
+
+Definition Microbenchmarks_Carrier : Type := sum (list W) (list (list W)).
+
+Definition Microbenchmarks_Env : Env Microbenchmarks_Carrier :=
+  (GLabelMap.empty (FuncSpec _))
+    ### ("std", "rand") ->> (Axiomatic FRandom)
+    ### ("list", "nil") ->> (Axiomatic (FacadeImplementationOfConstructor (list W) nil))
+    ### ("list[W]", "push") ->> (Axiomatic (FacadeImplementationOfMutation_SCA (list W) cons))
+    ### ("list[W]", "pop") ->> (Axiomatic (List_pop W))
+    ### ("list[W]", "delete") ->> (Axiomatic (FacadeImplementationOfDestructor (list W)))
+    ### ("list[W]", "empty?") ->> (Axiomatic (List_empty W))
+    ### ("list[list[W]]", "nil") ->> (Axiomatic (FacadeImplementationOfConstructor (list (list W)) nil))
+    ### ("list[list[W]]", "push") ->> (Axiomatic (FacadeImplementationOfMutation_ADT (list W) (list (list W)) cons))
+    ### ("list[list[W]]", "pop") ->> (Axiomatic (List_pop (list W)))
+    ### ("list[list[W]]", "delete") ->> (Axiomatic (FacadeImplementationOfDestructor (list (list W))))
+    ### ("list[list[W]]", "empty?") ->> (Axiomatic (List_empty (list W))).
+
+Notation "'ParametricExtraction' '#vars' x .. y '#program' post '#arguments' pre '#env' env '#carrier' carrier" :=
+  (sigT (fun prog => (forall x, .. (forall y, {{ pre }} prog {{ [[`"out" <~~ post as _]]::Nil }} ∪ {{ ∅ }} // (env: Env carrier)) ..)))
+    (at level 200,
+     x binder,
+     y binder,
+     format "'ParametricExtraction' '//'    '#vars'       x .. y '//'    '#program'     post '//'    '#arguments'  pre '//'    '#env'        env '//'    '#carrier'    carrier").
+
+Notation "'ParametricExtraction' '#vars' x .. y '#program' post '#arguments' pre '#env' env" :=
+  (sigT (fun prog => (forall x, .. (forall y, {{ pre }} prog {{ [[`"out" <~~ post as _]]::Nil }} ∪ {{ ∅ }} // env) ..)))
+    (at level 200,
+     x binder,
+     y binder,
+     format "'ParametricExtraction' '//'    '#vars'       x .. y '//'    '#program'     post '//'    '#arguments'  pre '//'    '#env'         env").
+
+Notation "'ParametricExtraction' '#program' post '#env' env" :=
+  (sigT (fun prog => {{ Nil }} prog {{ [[`"out" <~~ post as _]]::Nil }} ∪ {{ ∅ }} // env))
+    (at level 200,
+     format "'ParametricExtraction' '//'    '#program'  post '//'    '#env'      env").
+
+Notation "'FacadeMethod' '#prog' prog '#requires' pre '#ensures' post '#ext' ext '#env' env" :=
+  ({{ pre }} prog {{ post }} ∪ {{ ext }} // env)
+    (at level 200,
+     format "'FacadeMethod' '//'    '#prog'      prog '//'    '#requires'  pre '//'    '#ensures'   post '//'    '#ext'       ext '//'    '#env'       env").
+
+Example micro_plus :
+  ParametricExtraction
+    #vars      x y
+    #program   ret (Word.wplus x y)
+    #arguments [[`"x" <-- x as _ ]] :: [[`"y" <-- y as _ ]] :: Nil
+    #env       Microbenchmarks_Env.
+Proof.
+  _compile.
+Defined.
+
+Time Eval lazy in (extract_facade micro_plus).
+
+Example micro_plus_minus :
+  ParametricExtraction
+    #vars      x y
+    #program   ret (Word.wplus x (Word.wminus y x))
+    #arguments [[`"x" <-- x as _ ]] :: [[`"y" <-- y as _ ]] :: Nil
+    #env       Microbenchmarks_Env.
+Proof.
+  repeat (_compile_step || apply ProgOk_Chomp_Some_snd).
+Defined.
+
+Time Eval lazy in (extract_facade micro_plus_minus).
+
+Example micro_min :
+  ParametricExtraction
+    #vars      x y
+    #program   ret (if Word.wlt_dec x y then x else y)
+    #arguments [[`"x" <-- x as _ ]] :: [[`"y" <-- y as _ ]] :: Nil
+    #env       Microbenchmarks_Env.
+Proof.
+  _compile.
+Defined.
+
+Time Eval lazy in (extract_facade micro_min).
+
+Example micro_max :
+  ParametricExtraction
+    #vars      x y
+    #program   ret (if Word.wlt_dec x y then y else x)
+    #arguments [[`"x" <-- x as _ ]] :: [[`"y" <-- y as _ ]] :: Nil
+    #env       Microbenchmarks_Env.
+Proof.
+  _compile.
+Defined.
+
+Time Eval lazy in (extract_facade micro_max).
+
+Example micro_squared_max :
+  ParametricExtraction
+    #vars      x y
+    #program   ret (if Word.wlt_dec x y then Word.wmult y y else Word.wmult x x)
+    #arguments [[`"x" <-- x as _ ]] :: [[`"y" <-- y as _ ]] :: Nil
+    #env       Microbenchmarks_Env.
+Proof.
+  _compile.
+Defined.
+
+Time Eval lazy in (extract_facade micro_squared_max).
+
+Example micro_make_singleton :
+  ParametricExtraction
+    #vars      x y
+    #program   ret (x :: y :: nil)
+    #arguments [[`"x" <-- x as _ ]] :: [[`"y" <-- y as _ ]] :: Nil
+    #env       Microbenchmarks_Env.
+Proof.
+  _compile.
+Defined.
+
+Time Eval lazy in (extract_facade micro_make_singleton).
+
+Example micro_duplicate_word :
+  ParametricExtraction
+    #vars      x
+    #program   ret (x :: x :: nil)
+    #arguments [[`"x" <-- x as _ ]] :: Nil
+    #env       Microbenchmarks_Env.
+Proof.
+  _compile.
+Defined.
+
+Time Eval lazy in (extract_facade micro_duplicate_word).
+
+Example micro_sort_pair_1 :
+  ParametricExtraction
+    #vars      x y
+    #program   ret (if Word.wlt_dec x y then x :: y :: nil else y :: x :: nil)
+    #arguments [[`"x" <-- x as _ ]] :: [[`"y" <-- y as _ ]] :: Nil
+    #env       Microbenchmarks_Env.
+Proof.
+  _compile.
+Defined.
+
+Time Eval lazy in (extract_facade micro_sort_pair_1).
+
+Example micro_sort_pair_2 :
+  ParametricExtraction
+    #vars      x y
+    #program   ret ((if Word.wlt_dec x y then x else y) :: (if Word.wlt_dec x y then y else x) :: nil)
+    #arguments [[`"x" <-- x as _ ]] :: [[`"y" <-- y as _ ]] :: Nil
+    #env       Microbenchmarks_Env.
+Proof.
+  _compile.
+Defined.
+
+Time Eval lazy in (extract_facade micro_sort_pair_2).
+
+Example micro_double :
+  ParametricExtraction
+    #vars      seq
+    #program   ret (revmap (fun w => Word.wmult w 2) seq)
+    #arguments [[`"seq" <-- seq as _ ]] :: Nil
+    #env       Microbenchmarks_Env.
+Proof.                               (* FIXME prove something for maps *)
+  _compile.
+Defined.
+
+Time Eval lazy in (extract_facade micro_double).
+
+Example micro_fold_plus :
+  ParametricExtraction
+    #vars      seq
+    #program   ret (fold_left (@Word.wplus 32) seq 0)
+    #arguments [[`"seq" <-- seq as _ ]] :: Nil
+    #env       Microbenchmarks_Env.
+Proof.
+  _compile.
+  instantiate (1 := Skip).
+  admit.
+  (* let fop := translate_op Word.wplus in (* FIXME *) *)
+  (* apply (CompileBinopOrTest_right_inPlace fop); compile_do_side_conditions. *)
+Defined.
+
+Time Eval lazy in (extract_facade micro_fold_plus).
+
+Example micro_fold_plus_x :
+  ParametricExtraction
+    #vars      seq x
+    #program   ret (fold_left (@Word.wplus 32) seq x)
+    #arguments [[`"seq" <-- seq as _ ]] :: [[`"x" <-- x as _ ]] :: Nil
+    #env       Microbenchmarks_Env.
+Proof.
+  _compile.
+  instantiate (1 := Skip).
+  admit.
+  (* let fop := translate_op Word.wplus in (* FIXME *) *)
+  (* apply (CompileBinopOrTest_right_inPlace fop); compile_do_side_conditions. *)
+Defined.
+
+Time Eval lazy in (extract_facade micro_fold_plus_x).
+
+Lemma List_rev_as_fold_generalized :
+  forall A l init,
+    @List.rev A l ++ init = fold_left (fun acc x => x :: acc) l init.
+Proof.
+  induction l; simpl; intros; [ | rewrite <- IHl, <- app_assoc ]; reflexivity.
+Qed.
+
+Lemma List_rev_as_fold :
+  forall A l, @List.rev A l = fold_left (fun acc x => x :: acc) l nil.
+Proof.
+  intros; rewrite <- (List_rev_as_fold_generalized _ nil), app_nil_r; reflexivity.
+Qed.
+
+Ltac _compile_early_hook ::= rewrite List_rev_as_fold.
+
+Example micro_fold_reverse :
+  ParametricExtraction
+    #vars      seq
+    #program   ret (List.rev seq)
+    #arguments [[`"seq" <-- seq as _ ]] :: Nil
+    #env       Microbenchmarks_Env.
+Proof.
+  _compile.
+Defined.
+
+Time Eval lazy in (extract_facade micro_fold_reverse).
+
+Example micro_fold_flatten_rev :
+  ParametricExtraction
+    #vars      seqs
+    #program   ret (fold_left (fun acc seq => fold_left (fun acc' x => x :: acc') seq acc) seqs nil)
+    #arguments [[`"seqs" <-- seqs as _ ]] :: Nil
+    #env       Microbenchmarks_Env.
+Proof.
+  _compile.
+Defined.
+
+Time Eval lazy in (extract_facade micro_fold_flatten_rev).
+
+Lemma ProgOk_Remove_Skip_L :
+  forall {av} ext (t1 t2: Telescope av) env prog,
+    {{ t1 }} (Seq Skip prog) {{ t2 }} ∪ {{ ext }} // env ->
+    {{ t1 }} prog {{ t2 }} ∪ {{ ext }} // env.
+Proof.
+  SameValues_Facade_t.
+  learn (RunsToSkip env (Equal_refl initial_state)); eauto.
+  learn (RunsToSeq (RunsToSkip _ (Equal_refl _)) H1); eauto.
+Qed.
+
+Lemma ProgOk_Remove_Skip_R :
+  forall {av} ext (t1 t2: Telescope av) env prog,
+    {{ t1 }} (Seq prog Skip) {{ t2 }} ∪ {{ ext }} // env ->
+    {{ t1 }} prog {{ t2 }} ∪ {{ ext }} // env.
+Proof.
+  SameValues_Facade_t.
+  learn (RunsToSeq H1 (RunsToSkip _ (Equal_refl _))); eauto.
+Qed.
+
+Lemma ProgOk_Transitivity_Name_SCA :
+  forall {av} k env ext t1 (t2: W -> Telescope av) prog1 (v: Comp W),
+    {{ t1 }} prog1 {{ [[`k <~~ v as kk]]::t2 kk }} ∪ {{ ext }} // env ->
+    {{ t1 }} prog1 {{ [[v as kk]]::t2 kk }} ∪ {{ ext }} // env.
+Proof.
+  SameValues_Facade_t.
+  eauto using SameValues_Dealloc_SCA.
+Qed.
+
+Ltac _compile_random :=
+  match_ProgOk
+    ltac:(fun prog pre post ext env =>
+            match constr:(pre, post) with
+            | (?tenv, Cons ?k Random ?tenv') =>
+              match k with
+              | NTNone => let vrandom := gensym "random" in
+                         apply ProgOk_Transitivity_Name_SCA with vrandom
+              | _ => idtac
+              end;
+                first [ call_tactic_after_moving_head_binding_to_separate_goal ltac:(apply CompileCallRandom)
+                      | apply miniChomp'; apply CompileDeallocSCA_discretely ]
+            end).
+
+Ltac _compile_early_hook ::= _compile_random.
+
+Example micro_pick_random :
+  ParametricExtraction
+    #program Random
+    #env     Microbenchmarks_Env.
+Proof.
+  _compile.
+Defined.
+
+Time Eval lazy in (extract_facade micro_pick_random).
+
+Example micro_sum_random :
+  ParametricExtraction
+    #program ( r1 <- Random;
+               r2 <- Random;
+               ret (Word.wplus r1 r2) )
+    #env     Microbenchmarks_Env.
+Proof.
+  _compile.
+Defined.
+
+Time Eval lazy in (extract_facade micro_sum_random).
+
+(* FIXME loops on zips? *)
+
+Example micro_randomize :
+  ParametricExtraction
+    #vars      seq: list W
+    #program   fold_left (fun acc elem => ( a <- acc;
+                                         r <- Random;
+                                         ret (r :: a) )%comp) seq (ret nil)
+    #arguments [[`"seq" <-- seq as _ ]] :: Nil
+    #env       Microbenchmarks_Env.
+Proof.
+  _compile.
+  apply miniChomp'.             (* FIXME *)
+  _compile.
+Defined.
+
+Time Eval lazy in (extract_facade micro_randomize).
+
+Example micro_double_larger_than_random :
+  ParametricExtraction
+    #vars      seq
+    #program   ( threshold <- Random;
+                 ret (revmap (fun w => if Word.wlt_dec threshold w then Word.wmult w 2 else w) seq) )
+    #arguments [[`"seq" <-- seq as _ ]] :: Nil
+    #env       Microbenchmarks_Env.
+Proof.                               (* FIXME prove something for maps *)
+  _compile.
+Defined.
+
+Time Eval lazy in (extract_facade micro_double_larger_than_random).
+
+Example micro_drop_larger_than_random :
+  ParametricExtraction
+    #vars      seq
+    #program   ( threshold <- Random;
+                 ret (fold_left (fun acc w => if Word.wlt_dec threshold w then acc else w :: acc) seq nil) )
+    #arguments [[`"seq" <-- seq as _ ]] :: Nil
+    #env       Microbenchmarks_Env.
+Proof.
+  _compile.
+Defined.
+
+Time Eval lazy in (extract_facade micro_drop_larger_than_random).
